trillium/program_logic/ectx_language.v
@@ -11,13 +11,17 @@ file for doing that. *)
 Section ectx_language_mixin.
   Context {expr val ectx state : Type}.
   Context {locale : Type}.
+  Context {action : Type}.
+  Context {config_label : Type}.
   Context (of_val : val → expr).
   Context (to_val : expr → option val).
   Context (empty_ectx : ectx).
   Context (comp_ectx : ectx → ectx → ectx).
   Context (fill : ectx → expr → expr).
-  Context (head_step : expr → state → expr → state → list expr → Prop).
-  Context (locale_of : list expr -> expr -> locale).
+  Context (head_step : expr → state → action → expr → state → list expr → Prop).
+  Context (config_step : state → config_label → state → Prop).
+  Context (locale_of : list expr → expr → locale).
+  Context (config_enabled : config_label → state → Prop).
 
   Notation locales_equiv t0 t0' :=
     (Forall2 (λ '(t, e) '(t', e'), locale_of t e = locale_of t' e') (prefixes t0) (prefixes t0')).
@@ -25,8 +29,8 @@ Section ectx_language_mixin.
   Record EctxLanguageMixin := {
     mixin_to_of_val v : to_val (of_val v) = Some v;
     mixin_of_to_val e v : to_val e = Some v → of_val v = e;
-    mixin_val_head_stuck e1 σ1 e2 σ2 efs :
-      head_step e1 σ1 e2 σ2 efs → to_val e1 = None;
+    mixin_val_head_stuck e1 σ1 α e2 σ2 efs :
+      head_step e1 σ1 α e2 σ2 efs → to_val e1 = None;
 
     mixin_fill_empty e : fill empty_ectx e = e;
     mixin_fill_comp K1 K2 e : fill K1 (fill K2 e) = fill (comp_ectx K1 K2) e;
@@ -45,23 +49,25 @@ Section ectx_language_mixin.
 
         This implies there can be only one head redex, see
         [head_redex_unique]. *)
-    mixin_step_by_val K' K_redex e1' e1_redex σ1 e2 σ2 efs :
+    mixin_step_by_val K' K_redex e1' e1_redex σ1 α  e2 σ2 efs :
       fill K' e1' = fill K_redex e1_redex →
       to_val e1' = None →
-      head_step e1_redex σ1 e2 σ2 efs →
+      head_step e1_redex σ1 α e2 σ2 efs →
       ∃ K'', K_redex = comp_ectx K' K'';
 
     (** If [fill K e] takes a head step, then either [e] is a value or [K] is
         the empty evaluation context. In other words, if [e] is not a value
         wrapping it in a context does not add new head redex positions. *)
-    mixin_head_ctx_step_val K e σ1 e2 σ2 efs :
-      head_step (fill K e) σ1 e2 σ2 efs → is_Some (to_val e) ∨ K = empty_ectx;
-    mixin_locale_step e1 e2 t1 σ1 σ2 efs: head_step e1 σ1 e2 σ2 efs ->
+    mixin_head_ctx_step_val K e σ1 α e2 σ2 efs :
+      head_step (fill K e) σ1 α e2 σ2 efs → is_Some (to_val e) ∨ K = empty_ectx;
+    mixin_locale_step e1 e2 t1 σ1 α σ2 efs: head_step e1 σ1 α e2 σ2 efs ->
                                          locale_of t1 e1 = locale_of t1 e2;
     mixin_locale_fill e K t1: locale_of t1 (fill K e) = locale_of t1 e;
     mixin_locale_equiv t t' e: locales_equiv t t' -> locale_of t e = locale_of t' e;
     mixin_locale_injective tp0 e0 tp1 tp e:
       (tp, e) ∈ prefixes_from (tp0 ++ [e0]) tp1 -> locale_of tp0 e0 ≠ locale_of tp e;
+    (* mixin_config_enabled σ lbl : *)
+    (*   (∃ σ', config_step σ lbl σ') ↔ config_enabled lbl σ; *)
   }.
 End ectx_language_mixin.
 
@@ -71,32 +77,36 @@ Structure ectxLanguage := EctxLanguage {
   ectx : Type;
   state : Type;
   locale : Type;
+  action : Type;
+  config_label : Type;
 
   of_val : val → expr;
   to_val : expr → option val;
   empty_ectx : ectx;
   comp_ectx : ectx → ectx → ectx;
   fill : ectx → expr → expr;
-  head_step : expr → state → expr → state → list expr → Prop;
-  config_step : state → state → Prop;
-  locale_of : list expr -> expr -> locale;
+  head_step : expr → state → action → expr → state → list expr → Prop;
+  config_step : state → config_label → state → Prop;
+  locale_of : list expr → expr → locale;
+  (* config_enabled : config_label → state → Prop; *)
 
   ectx_language_mixin :
-    EctxLanguageMixin of_val to_val empty_ectx comp_ectx fill head_step locale_of
+    EctxLanguageMixin of_val to_val empty_ectx comp_ectx fill head_step (* config_step *) locale_of (* config_enabled *)
 }.
 
 Bind Scope expr_scope with expr.
 Bind Scope val_scope with val.
 
-Arguments EctxLanguage {_ _ _ _ _ _ _ _ _ _} _ _.
+Arguments EctxLanguage {_ _ _ _ _ _ _ _ _ _ _ _} _ _ _.
 Arguments of_val {_} _.
 Arguments to_val {_} _.
 Arguments empty_ectx {_}.
 Arguments comp_ectx {_} _ _.
 Arguments fill {_} _ _.
 Arguments head_step {_} _ _ _ _ _.
-Arguments config_step {_} _ _.
+Arguments config_step {_} _ _ _.
 Arguments locale_of {_} _ _.
+(* Arguments config_enabled {_} _ _. *)
 
 Notation locales_equiv t0 t0' :=
   (Forall2 (λ '(t, e) '(t', e'), locale_of t e = locale_of t' e') (prefixes t0) (prefixes t0')).
@@ -109,7 +119,7 @@ Section ectx_language.
   Implicit Types K : ectx Λ.
 
   (* Only project stuff out of the mixin that is not also in language *)
-  Lemma val_head_stuck e1 σ1 e2 σ2 efs : head_step e1 σ1 e2 σ2 efs → to_val e1 = None.
+  Lemma val_head_stuck e1 σ1 α e2 σ2 efs : head_step e1 σ1 α e2 σ2 efs → to_val e1 = None.
   Proof. apply ectx_language_mixin. Qed.
   Lemma fill_empty e : fill empty_ectx e = e.
   Proof. apply ectx_language_mixin. Qed.
@@ -124,20 +134,20 @@ Section ectx_language.
     fill K e = fill K' e' →
     (∃ K'', K' = comp_ectx K K'') ∨ (∃ K'', K = comp_ectx K' K'').
   Proof. apply ectx_language_mixin. Qed.
-  Lemma step_by_val K' K_redex e1' e1_redex σ1 e2 σ2 efs :
+  Lemma step_by_val K' K_redex e1' e1_redex σ1 α e2 σ2 efs :
       fill K' e1' = fill K_redex e1_redex →
       to_val e1' = None →
-      head_step e1_redex σ1 e2 σ2 efs →
+      head_step e1_redex σ1 α e2 σ2 efs →
       ∃ K'', K_redex = comp_ectx K' K''.
   Proof. apply ectx_language_mixin. Qed.
-  Lemma head_ctx_step_val K e σ1 e2 σ2 efs :
-    head_step (fill K e) σ1 e2 σ2 efs → is_Some (to_val e) ∨ K = empty_ectx.
+  Lemma head_ctx_step_val K e σ1 α e2 σ2 efs :
+    head_step (fill K e) σ1 α e2 σ2 efs → is_Some (to_val e) ∨ K = empty_ectx.
   Proof. apply ectx_language_mixin. Qed.
 
   Definition head_reducible (e : expr Λ) (σ : state Λ) :=
-    ∃ e' σ' efs, head_step e σ e' σ' efs.
+    ∃ α e' σ' efs, head_step e σ α e' σ' efs.
   Definition head_irreducible (e : expr Λ) (σ : state Λ) :=
-    ∀ e' σ' efs, ¬head_step e σ e' σ' efs.
+    ∀ α e' σ' efs, ¬head_step e σ α e' σ' efs.
   Definition head_stuck (e : expr Λ) (σ : state Λ) :=
     to_val e = None ∧ head_irreducible e σ.
 
@@ -149,33 +159,33 @@ Section ectx_language.
   Definition sub_redexes_are_values (e : expr Λ) :=
     ∀ K e', e = fill K e' → to_val e' = None → K = empty_ectx.
 
-  Inductive prim_step (e1 : expr Λ) (σ1 : state Λ)
+  Inductive prim_step (e1 : expr Λ) (σ1 : state Λ) (α : action Λ) 
       (e2 : expr Λ) (σ2 : state Λ) (efs : list (expr Λ)) : Prop :=
     Ectx_step K e1' e2' :
       e1 = fill K e1' → e2 = fill K e2' →
-      head_step e1' σ1 e2' σ2 efs → prim_step e1 σ1 e2 σ2 efs.
+      head_step e1' σ1 α e2' σ2 efs → prim_step e1 σ1 α e2 σ2 efs.
 
-  Lemma Ectx_step' K e1 σ1 e2 σ2 efs :
-    head_step e1 σ1 e2 σ2 efs → prim_step (fill K e1) σ1 (fill K e2) σ2 efs.
+  Lemma Ectx_step' K e1 σ1 α e2 σ2 efs :
+    head_step e1 σ1 α e2 σ2 efs → prim_step (fill K e1) σ1 α (fill K e2) σ2 efs.
   Proof. econstructor; eauto. Qed.
 
   Lemma fill_not_val K e : to_val e = None → to_val (fill K e) = None.
   Proof. rewrite !eq_None_not_Some. eauto using fill_val. Qed.
 
   Definition ectx_lang_mixin :
-    LanguageMixin of_val to_val prim_step locale_of comp_ectx empty_ectx fill.
+    LanguageMixin of_val to_val prim_step (* config_step *) locale_of (* config_enabled *) comp_ectx empty_ectx fill.
   Proof.
     split.
     - apply ectx_language_mixin.
     - apply ectx_language_mixin.
-    - intros ????? [??? -> -> ?%val_head_stuck].
+    - intros ?????? [??? -> -> ?%val_head_stuck].
       apply eq_None_not_Some. by intros ?%fill_val%eq_None_not_Some.
     - intros K; split_and!.
       + eauto using fill_not_val.
-      + intros ????? [K' e1' e2' Heq1 Heq2 Hstep].
+      + intros ?????? [K' e1' e2' Heq1 Heq2 Hstep].
         exists (comp_ectx K K') e1' e2'; rewrite ?Heq1 ?Heq2 ?fill_comp; done.
-      + intros e1 σ1 e2 σ2 efs Hnval [K'' e1'' e2'' Heq1 -> Hstep].
-        destruct (step_by_val K K'' e1 e1'' σ1 e2'' σ2 efs) as [K' ->]; eauto.
+      + intros e1 σ1 α e2 σ2 efs Hnval [K'' e1'' e2'' Heq1 -> Hstep].
+        destruct (step_by_val K K'' e1 e1'' σ1 α e2'' σ2 efs) as [K' ->]; eauto.
         rewrite -fill_comp in Heq1; apply (inj (fill _)) in Heq1.
         exists (fill K' e2''); rewrite -fill_comp; split; auto.
         econstructor; eauto.
@@ -183,25 +193,27 @@ Section ectx_language.
     - intros ? ? ?; rewrite fill_comp; done.
     - apply fill_inj.
     - apply fill_positive.
-    - intros e1 e2 t1 σ1 σ2 efs Hpstep. inversion Hpstep; simplify_eq.
+    - intros e1 e2 α t1 σ1 σ2 efs Hpstep. inversion Hpstep; simplify_eq.
       do 2 (erewrite mixin_locale_fill; last apply ectx_language_mixin).
       eapply mixin_locale_step; first apply ectx_language_mixin. done.
     - apply ectx_language_mixin.
     - apply ectx_language_mixin.
     - apply ectx_language_mixin.
+    (* - apply ectx_language_mixin. *)
   Qed.
 
   Canonical Structure ectx_lang : language :=
-    Language (config_step := config_step) prim_step empty_ectx fill ectx_lang_mixin.
+    Language prim_step config_step (* (config_enabled := config_enabled) *)
+             empty_ectx fill ectx_lang_mixin.
 
   Definition head_atomic (a : atomicity) (e : expr Λ) : Prop :=
-    ∀ σ e' σ' efs,
-      head_step e σ e' σ' efs →
+    ∀ σ α e' σ' efs,
+      head_step e σ α e' σ' efs →
       if a is WeaklyAtomic then irreducible e' σ' else is_Some (to_val e').
 
   Definition head_stutteringatomic (a : atomicity) (e : expr Λ) : Prop :=
-    ∀ σ e' σ' efs,
-      head_step e σ e' σ' efs →
+    ∀ σ α e' σ' efs,
+      head_step e σ α e' σ' efs →
       (e' = e ∧ σ' = σ ∧ efs = [])
       ∨
       if a is WeaklyAtomic then irreducible e' σ' else is_Some (to_val e').
@@ -220,35 +232,35 @@ Section ectx_language.
     head_reducible e' σ →
     K = comp_ectx K' empty_ectx ∧ e = e'.
   Proof.
-    intros Heq (e2 & σ2 & efs & Hred) (e2' & σ2' & efs' & Hred').
+    intros Heq (α & e2 & σ2 & efs & Hred) (α' & e2' & σ2' & efs' & Hred').
     edestruct (step_by_val K' K e' e) as [K'' HK];
       [by eauto using val_head_stuck..|].
     subst K. move: Heq. rewrite -fill_comp. intros <-%(inj (fill _)).
-    destruct (head_ctx_step_val _ _ _ _ _ _ Hred') as [[]%not_eq_None_Some|HK''].
+    destruct (head_ctx_step_val _ _ _ _ _ _ _ Hred') as [[]%not_eq_None_Some|HK''].
     { by eapply val_head_stuck. }
     subst K''. rewrite fill_empty. done.
   Qed.
 
-  Lemma head_prim_step e1 σ1 e2 σ2 efs :
-    head_step e1 σ1 e2 σ2 efs → prim_step e1 σ1 e2 σ2 efs.
+  Lemma head_prim_step e1 σ1 α e2 σ2 efs :
+    head_step e1 σ1 α e2 σ2 efs → prim_step e1 σ1 α e2 σ2 efs.
   Proof. apply Ectx_step with empty_ectx; by rewrite ?fill_empty. Qed.
 
-  Lemma head_step_not_stuck e σ e' σ' efs : head_step e σ e' σ' efs → not_stuck e σ.
+  Lemma head_step_not_stuck e σ α e' σ' efs : head_step e σ α e' σ' efs → not_stuck e σ.
   Proof. rewrite /not_stuck /reducible /=. eauto 10 using head_prim_step. Qed.
 
-  Lemma fill_prim_step K e1 σ1 e2 σ2 efs :
-    prim_step e1 σ1 e2 σ2 efs → prim_step (fill K e1) σ1 (fill K e2) σ2 efs.
+  Lemma fill_prim_step K e1 σ1 α e2 σ2 efs :
+    prim_step e1 σ1 α e2 σ2 efs → prim_step (fill K e1) σ1 α (fill K e2) σ2 efs.
   Proof.
     destruct 1 as [K' e1' e2' -> ->].
     rewrite !fill_comp. by econstructor.
   Qed.
   Lemma fill_reducible K e σ : reducible e σ → reducible (fill K e) σ.
   Proof.
-    intros (e'&σ'&efs&?). exists (fill K e'), σ', efs.
+    intros (α&e'&σ'&efs&?). exists α, (fill K e'), σ', efs.
     by apply fill_prim_step.
   Qed.
   Lemma head_prim_reducible e σ : head_reducible e σ → reducible e σ.
-  Proof. intros (e'&σ'&efs&?). eexists e', σ', efs. by apply head_prim_step. Qed.
+  Proof. intros (α&e'&σ'&efs&?). eexists α, e', σ', efs. by apply head_prim_step. Qed.
   Lemma head_prim_fill_reducible e K σ :
     head_reducible e σ → reducible (fill K e) σ.
   Proof. intro. by apply fill_reducible, head_prim_reducible. Qed.
@@ -260,7 +272,7 @@ Section ectx_language.
   Lemma prim_head_reducible e σ :
     reducible e σ → sub_redexes_are_values e → head_reducible e σ.
   Proof.
-    intros (e'&σ'&efs&[K e1' e2' -> -> Hstep]) ?.
+    intros (α&e'&σ'&efs&[K e1' e2' -> -> Hstep]) ?.
     assert (K = empty_ectx) as -> by eauto 10 using val_head_stuck.
     rewrite fill_empty /head_reducible; eauto.
   Qed.
@@ -280,7 +292,7 @@ Section ectx_language.
   Lemma ectx_language_atomic a e :
     head_atomic a e → sub_redexes_are_values e → Atomic a e.
   Proof.
-    intros Hatomic_step Hatomic_fill σ e' σ' efs [K e1' e2' -> -> Hstep].
+    intros Hatomic_step Hatomic_fill σ α e' σ' efs [K e1' e2' -> -> Hstep].
     assert (K = empty_ectx) as -> by eauto 10 using val_head_stuck.
     rewrite fill_empty. eapply Hatomic_step. by rewrite fill_empty.
   Qed.
@@ -288,18 +300,18 @@ Section ectx_language.
   Lemma ectx_language_stutteringatomic a e :
     head_stutteringatomic a e → sub_redexes_are_values e → StutteringAtomic a e.
   Proof.
-    intros Hatomic_step Hatomic_fill σ e' σ' efs [K e1' e2' -> -> Hstep].
+    intros Hatomic_step Hatomic_fill σ α e' σ' efs [K e1' e2' -> -> Hstep].
     assert (K = empty_ectx) as -> by eauto 10 using val_head_stuck.
     revert Hatomic_step; rewrite !fill_empty; intros Hatomic_step.
     eapply Hatomic_step; done.
   Qed.
 
-  Lemma head_reducible_prim_step_ctx K e1 σ1 e2 σ2 efs :
+  Lemma head_reducible_prim_step_ctx K e1 σ1 α e2 σ2 efs :
     head_reducible e1 σ1 →
-    prim_step (fill K e1) σ1 e2 σ2 efs →
-    ∃ e2', e2 = fill K e2' ∧ head_step e1 σ1 e2' σ2 efs.
+    prim_step (fill K e1) σ1 α e2 σ2 efs →
+    ∃ e2', e2 = fill K e2' ∧ head_step e1 σ1 α e2' σ2 efs.
   Proof.
-    intros (e2''&σ2''&efs''&HhstepK) [K' e1' e2' HKe1 -> Hstep].
+    intros (α''&e2''&σ2''&efs''&HhstepK) [K' e1' e2' HKe1 -> Hstep].
     edestruct (step_by_val K) as [K'' ?];
       eauto using val_head_stuck; simplify_eq/=.
     rewrite -fill_comp in HKe1; simplify_eq.
@@ -309,10 +321,10 @@ Section ectx_language.
     by rewrite !fill_empty.
   Qed.
 
-  Lemma head_reducible_prim_step e1 σ1 e2 σ2 efs :
+  Lemma head_reducible_prim_step e1 σ1 α e2 σ2 efs :
     head_reducible e1 σ1 →
-    prim_step e1 σ1 e2 σ2 efs →
-    head_step e1 σ1 e2 σ2 efs.
+    prim_step e1 σ1 α e2 σ2 efs →
+    head_step e1 σ1 α e2 σ2 efs.
   Proof.
     intros.
     edestruct (head_reducible_prim_step_ctx empty_ectx) as (?&?&?);
@@ -322,16 +334,16 @@ Section ectx_language.
 
   Record pure_head_step (e1 e2 : expr Λ) := {
     pure_head_step_safe σ1 : head_reducible e1 σ1;
-    pure_head_step_det σ1 e2' σ2 efs :
-      head_step e1 σ1 e2' σ2 efs → σ2 = σ1 ∧ e2' = e2 ∧ efs = []
+    pure_head_step_det σ1 α e2' σ2 efs :
+      head_step e1 σ1 α e2' σ2 efs → σ2 = σ1 ∧ e2' = e2 ∧ efs = []
   }.
 
   Lemma pure_head_step_pure_step e1 e2 : pure_head_step e1 e2 → pure_step e1 e2.
   Proof.
     intros [Hp1 Hp2]. split.
-    - intros σ. destruct (Hp1 σ) as (e2' & σ2 & efs & ?).
-      eexists e2', σ2, efs. by apply head_prim_step.
-    - intros σ1 e2' σ2 efs ?%head_reducible_prim_step; eauto.
+    - intros σ. destruct (Hp1 σ) as (α & e2' & σ2 & efs & ?).
+      eexists α, e2', σ2, efs. by apply head_prim_step.
+    - intros σ1 α e2' σ2 efs ?%head_reducible_prim_step; eauto.
   Qed.
 
   (** This is not an instance because HeapLang's [wp_pure] tactic already takes
@@ -344,11 +356,11 @@ Section ectx_language.
     PureExec φ n (fill K e1) (fill K e2).
   Proof. apply: pure_exec_ctx. Qed.
 
-  Lemma head_locale_step K e1 e2 tp1 tp2 efs σ1 σ2 :
-    head_step e1 σ1 e2 σ2 efs →
+  Lemma head_locale_step K e1 e2 α tp1 tp2 efs σ1 σ2 :
+    head_step e1 σ1 α e2 σ2 efs →
     locale_step
       (tp1 ++ fill K e1 :: tp2, σ1)
-      (Some (locale_of tp1 e1))
+      (inl (locale_of tp1 e1, α))
       (tp1 ++ fill K e2 :: tp2 ++ efs, σ2).
   Proof.
     intros Hstep. rewrite -(locale_fill _ K). econstructor =>//.
@@ -368,7 +380,7 @@ work.
 Note that this trick no longer works when we switch to canonical projections
 because then the pattern match [let '...] will be desugared into projections. *)
 Definition LanguageOfEctx (Λ : ectxLanguage) : language :=
-  let '@EctxLanguage E V C St Loc of_val to_val empty comp fill head config loc_of mix := Λ in
-  @Language E V C St Loc of_val to_val _ config loc_of comp empty fill
+  let '@EctxLanguage E V C St Loc locale action of_val to_val empty comp fill head config loc_of (* config_enabled *) mix := Λ in
+  @Language E V C St Loc locale action of_val to_val _ config loc_of (* config_enabled  *) comp empty fill
     (@ectx_lang_mixin
-       (@EctxLanguage E V C St Loc of_val to_val empty comp fill head config loc_of mix)).
+       (@EctxLanguage E V C St Loc locale action of_val to_val empty comp fill head config loc_of (* config_enabled *) mix)).
