fairneris/adequacy.v
@@ -1,0 +1,663 @@
+From Paco Require Import pacotac.
+From stdpp Require Import finite.
+From iris.proofmode Require Import proofmode.
+From trillium Require Import adequacy.
+From fairneris Require Import fairness model_draft.
+From fairneris.aneris_lang Require Import aneris_lang resources.
+From fairneris.aneris_lang.state_interp Require Import state_interp_def.
+From fairneris.aneris_lang.state_interp Require Import state_interp_config_wp.
+From fairneris.aneris_lang.state_interp Require Import state_interp.
+From fairneris.aneris_lang.program_logic Require Import aneris_weakestpre.
+From fairneris Require Import from_locale_utils.
+
+(* TODO: Move to stdpp *)
+Lemma gset_union_difference_intersection_L `{Countable A} (X Y : gset A) :
+  X = (X ∖ Y) ∪ (X ∩ Y).
+Proof. rewrite union_intersection_l_L difference_union_L. set_solver. Qed.
+
+(* TODO: Move *)
+Definition tr_starts_in {S L} (tr : trace S L) (s : S) := trfirst tr = s.
+
+Definition extrace_property {Λ} (c : cfg Λ) (Φ : extrace Λ → Prop) :=
+  ∀ extr, tr_starts_in extr c → extrace_valid extr → Φ extr.
+
+Lemma extrace_property_impl {Λ} c (Φ Ψ : extrace Λ → Prop) :
+  extrace_property c Φ →
+  (∀ extr, tr_starts_in extr c → extrace_valid extr → Φ extr → Ψ extr) →
+  extrace_property c Ψ.
+Proof. intros HΦ Himpl extr Hstarts Hvalid. by apply Himpl, HΦ. Qed.
+
+(* TODO: This is not used right now - Remove/Reintroduce? *)
+(* Definition always_holds {Σ} *)
+(*            `{!anerisG (fair_model_to_model simple_fair_model) Σ} *)
+(*            (s : stuckness) (ξ : execution_trace aneris_lang → *)
+(*                               finite_trace simple_state simple_role → Prop) *)
+(*            (c1 : cfg aneris_lang) *)
+(*            (c2 : (fair_model_to_model simple_fair_model).(mstate)) : iProp Σ := *)
+(*   ∀ ex atr c, *)
+(*     ⌜valid_system_trace ex atr⌝ -∗ *)
+(*     ⌜trace_starts_in ex c1⌝ -∗ *)
+(*     ⌜trace_starts_in atr c2⌝ -∗ *)
+(*     ⌜trace_ends_in ex c⌝ -∗ *)
+(*     ⌜∀ ex' atr' oζ ℓ, trace_contract ex oζ ex' → *)
+(*                       trace_contract atr ℓ atr' → ξ ex' atr'⌝ -∗ *)
+(*     ⌜∀ e2, s = NotStuck → e2 ∈ c.1 → not_stuck e2 c.2⌝ -∗ *)
+(*     state_interp ex atr -∗ *)
+(*     |={⊤, ∅}=> ⌜ξ ex atr⌝. *)
+
+(* TODO: Clean up this definition (annoying to state lemmas about,
+         due to separate labels) *)
+Definition live_tid (c : cfg aneris_lang) (δ : simple_state)
+  (ℓ:fmrole simple_fair_model) (ζ:ex_label aneris_lang) : Prop :=
+  labels_match ζ ℓ → role_enabled_model ℓ δ → live_ex_label ζ c.
+
+Definition live_tids (c : cfg aneris_lang) (δ : simple_state) : Prop :=
+  ∀ ℓ ζ, live_tid c δ ℓ ζ.
+
+Definition valid_state_evolution_fairness
+           (extr : execution_trace aneris_lang)
+           (auxtr : auxiliary_trace (fair_model_to_model simple_fair_model)) :=
+  auxtr_valid auxtr ∧
+  labels_match_trace extr auxtr ∧
+  live_tids (trace_last extr) (trace_last auxtr).
+
+Lemma rel_finitary_valid_state_evolution_fairness :
+  rel_finitary valid_state_evolution_fairness.
+Proof. Admitted.
+
+Definition locale_dead_role_disabled (c : cfg aneris_lang)
+           (δ : simple_state) :=
+  ∀ (ℓ:fmrole simple_fair_model) ζ,
+  labels_match (inl ζ) ℓ →
+  ∀ e, from_locale c.1 ζ = Some e → is_Some (language.to_val e) →
+       ¬ role_enabled_model ℓ δ.
+
+Lemma derive_live_tid_inl c δ (ℓ : fmrole simple_fair_model) ζ :
+  role_enabled_locale_exists c δ →
+  locale_dead_role_disabled c δ →
+  live_tid c δ ℓ (inl ζ).
+Proof.
+  intros Himpl1 Himpl2 Hmatch Hrole.
+  specialize (Himpl1 _ _ Hmatch Hrole) as [e He].
+  exists e.
+  split; [done|].
+  destruct (language.to_val e) eqn:Heqn; [|done].
+  specialize (Himpl2 _ _ Hmatch e He).
+  assert (is_Some $ language.to_val e) as Hsome by done.
+  by specialize (Himpl2 Hsome).
+Qed.
+
+Lemma derive_live_tid_inr (c : cfg aneris_lang) δ
+      (ℓ : fmrole simple_fair_model) ζ :
+  config_state_valid c δ → live_tid c δ ℓ (inr ζ).
+Proof.
+  intros (Hn&Hm) Hlabels.
+  assert (ℓ ≠ A_role ∧ ℓ ≠ B_role) as [HAneq HBneq].
+  { rewrite /labels_match /locale_simple_label in Hlabels.
+    repeat case_match; simplify_eq; eauto. }
+  intros Henabled.
+  rewrite /role_enabled_model in Henabled.
+  destruct δ eqn:Heq; simpl in *.
+  + set_solver.
+  + destruct ℓ.
+    * by destruct sent; set_solver.
+    * by destruct sent; set_solver.
+    * destruct sent; [by set_solver|].
+      assert (ζ = DuplicateLabel) as ->.
+      { rewrite /labels_match /locale_simple_label in Hlabels.
+        by repeat case_match; simplify_eq. }
+      simpl. rewrite /config_enabled. rewrite Hn.
+      simpl.
+      rewrite gmultiset_disj_union_comm.
+      intros Hneq.
+      assert (mAB ∈ {[+ mAB +]} ⊎ mABn sent) by multiset_solver.
+      rewrite Hneq in H.
+      set_solver.
+    * destruct sent; [by set_solver|].
+      assert (ζ = DropLabel) as ->.
+      { rewrite /labels_match /locale_simple_label in Hlabels.
+        by repeat case_match; simplify_eq. }
+      simpl. rewrite /config_enabled. rewrite Hn.
+      simpl.
+      rewrite gmultiset_disj_union_comm.
+      intros Hneq.
+      assert (mAB ∈ {[+ mAB +]} ⊎ mABn sent) by multiset_solver.
+      rewrite Hneq in H.
+      set_solver.
+    * destruct sent; [by set_solver|].
+      assert (ζ = DeliverLabel) as ->.
+      { rewrite /labels_match /locale_simple_label in Hlabels.
+        by repeat case_match; simplify_eq. }
+      simpl. rewrite /config_enabled. rewrite Hn.
+      simpl.
+      rewrite gmultiset_disj_union_comm.
+      intros Hneq.
+      assert (mAB ∈ {[+ mAB +]} ⊎ mABn sent) by multiset_solver.
+      rewrite Hneq in H.
+      set_solver.
+  + destruct ℓ.
+    * by destruct sent; set_solver.
+    * by destruct sent; set_solver.
+    * destruct sent; [by set_solver|].
+      assert (ζ = DuplicateLabel) as ->.
+      { rewrite /labels_match /locale_simple_label in Hlabels.
+        by repeat case_match; simplify_eq. }
+      simpl. rewrite /config_enabled. rewrite Hn.
+      simpl.
+      rewrite gmultiset_disj_union_comm.
+      intros Hneq.
+      assert (mAB ∈ {[+ mAB +]} ⊎ mABn sent) by multiset_solver.
+      rewrite Hneq in H.
+      set_solver.
+    * destruct sent; [by set_solver|].
+      assert (ζ = DropLabel) as ->.
+      { rewrite /labels_match /locale_simple_label in Hlabels.
+        by repeat case_match; simplify_eq. }
+      simpl. rewrite /config_enabled. rewrite Hn.
+      simpl.
+      rewrite gmultiset_disj_union_comm.
+      intros Hneq.
+      assert (mAB ∈ {[+ mAB +]} ⊎ mABn sent) by multiset_solver.
+      rewrite Hneq in H.
+      set_solver.
+    * destruct sent; [by set_solver|].
+      assert (ζ = DeliverLabel) as ->.
+      { rewrite /labels_match /locale_simple_label in Hlabels.
+        by repeat case_match; simplify_eq. }
+      simpl. rewrite /config_enabled. rewrite Hn.
+      simpl.
+      rewrite gmultiset_disj_union_comm.
+      intros Hneq.
+      assert (mAB ∈ {[+ mAB +]} ⊎ mABn sent) by multiset_solver.
+      rewrite Hneq in H.
+      set_solver.
+  + destruct ℓ.
+    * by destruct sent; set_solver.
+    * by destruct sent; set_solver.
+    * destruct sent; [by set_solver|].
+      assert (ζ = DuplicateLabel) as ->.
+      { rewrite /labels_match /locale_simple_label in Hlabels.
+        by repeat case_match; simplify_eq. }
+      simpl. rewrite /config_enabled. rewrite Hn.
+      simpl.
+      rewrite gmultiset_disj_union_comm.
+      intros Hneq.
+      assert (mAB ∈ {[+ mAB +]} ⊎ mABn sent) by multiset_solver.
+      rewrite Hneq in H.
+      set_solver.
+    * destruct sent; [by set_solver|].
+      assert (ζ = DropLabel) as ->.
+      { rewrite /labels_match /locale_simple_label in Hlabels.
+        by repeat case_match; simplify_eq. }
+      simpl. rewrite /config_enabled. rewrite Hn.
+      simpl.
+      rewrite gmultiset_disj_union_comm.
+      intros Hneq.
+      assert (mAB ∈ {[+ mAB +]} ⊎ mABn sent) by multiset_solver.
+      rewrite Hneq in H.
+      set_solver.
+    * destruct sent; [by set_solver|].
+      assert (ζ = DeliverLabel) as ->.
+      { rewrite /labels_match /locale_simple_label in Hlabels.
+        by repeat case_match; simplify_eq. }
+      simpl. rewrite /config_enabled. rewrite Hn.
+      simpl.
+      rewrite gmultiset_disj_union_comm.
+      intros Hneq.
+      assert (mAB ∈ {[+ mAB +]} ⊎ mABn sent) by multiset_solver.
+      rewrite Hneq in H.
+      set_solver.
+Qed.
+
+Lemma valid_state_live_tids ex atr :
+  simple_valid_state_evolution ex atr →
+  locale_dead_role_disabled (trace_last ex) (trace_last atr) →
+  live_tids (trace_last ex) (trace_last atr).
+Proof.
+  intros (_&_&Hlive1&Hnm) Hlive2.
+  intros ℓ ζ Hlabels.
+  destruct ζ as [ζ|ζ].
+  - by apply derive_live_tid_inl.
+  - by apply derive_live_tid_inr.
+Qed.
+
+Definition continued_simulation_init {Λ M}
+           (ξ : execution_trace Λ → auxiliary_trace M → Prop)
+           (c : cfg Λ) (s : mstate M) :=
+  continued_simulation ξ {tr[c]} {tr[s]}.
+
+Definition wp_proto `{anerisPreG simple_fair_model Σ} IPs A
+           lbls obs_send_sas obs_rec_sas s es ip st :=
+  (∀ (aG : anerisG simple_fair_model Σ), ⊢ |={⊤}=>
+     unallocated A -∗
+     ([∗ set] a ∈ A, a ⤳[bool_decide (a ∈ obs_send_sas), bool_decide (a ∈ obs_rec_sas)] (∅, ∅)) -∗
+     live_roles_frag_own (simple_live_roles st ∖ config_roles) -∗
+     dead_roles_frag_own ((all_roles ∖ simple_live_roles st) ∖ config_roles) -∗
+     ([∗ set] i ∈ IPs, free_ip i) -∗
+     is_node ip -∗
+     ([∗ set] lbl ∈ lbls, alloc_evs lbl []) -∗
+     ([∗ set] sa ∈ obs_send_sas, sendon_evs sa []) -∗
+     ([∗ set] sa ∈ obs_rec_sas, receiveon_evs sa []) -∗
+     observed_send obs_send_sas -∗
+     observed_receive obs_rec_sas ={⊤}=∗
+     wptp s es (map (λ '(tnew,e), λ v, fork_post (locale_of tnew e) v)
+                    (prefixes es))
+     (* OBS: Can add [always_holds ξ] here *)).
+
+Theorem strong_simulation_adequacy_multiple Σ
+    `{!anerisPreG simple_fair_model Σ}
+    (s : stuckness) (es : list aneris_expr) (σ : state) (st : simple_state)
+    A obs_send_sas obs_rec_sas IPs ip lbls :
+  length es ≥ 1 →
+  role_enabled_locale_exists (es, σ) st →
+  state_ms σ = mABn (state_get_n st) →
+  (∃ shA shB : socket_handle,
+      state_sockets σ =
+      {[ipA := {[shA := (sA, [])]};
+        ipB := {[shB := (sB, mABm (state_get_m st))]}]}) →
+  wp_proto IPs A lbls obs_send_sas obs_rec_sas s es ip st →
+  obs_send_sas ⊆ A → obs_rec_sas ⊆ A →
+  ip ∉ IPs →
+  dom (state_ports_in_use σ) = IPs →
+  (∀ ip, ip ∈ IPs → state_ports_in_use σ !! ip = Some ∅) →
+  (∀ a, a ∈ A → ip_of_address a ∈ IPs) →
+  state_heaps σ = {[ip:=∅]} →
+  state_sockets σ = {[ip:=∅]} →
+  state_ms σ = ∅ →
+  continued_simulation_init valid_state_evolution_fairness (es, σ) st.
+Proof.
+  intros Hlen Hlive HmABn HmABm Hwp Hsendle Hrecvle Hipdom Hpiiu Hip Hfixdom Hste Hsce Hmse.
+  apply (wp_strong_adequacy_multiple aneris_lang (fair_model_to_model simple_fair_model) Σ s);
+    [done| |].
+  { apply rel_finitary_valid_state_evolution_fairness. }
+  iIntros (?) "".
+  iMod node_gnames_auth_init as (γmp) "Hmp".
+  iMod saved_si_init as (γsi) "[Hsi Hsi']".
+  iMod (unallocated_init (to_singletons A)) as (γsif)
+    "[Hunallocated_auth Hunallocated]".
+  iMod (free_ips_init IPs) as (γips) "[HIPsCtx HIPs]".
+  iMod free_ports_auth_init as (γpiu) "HPiu".
+  iMod (allocated_address_groups_init (to_singletons obs_send_sas)) as
+      (γobserved_send) "#Hobserved_send".
+  iMod (allocated_address_groups_init (to_singletons obs_rec_sas)) as
+      (γobserved_receive) "#Hobserved_receive".
+  iMod (socket_address_group_ctx_init (to_singletons A)) as (γC) "Hauth";
+    [apply to_singletons_all_disjoint|].
+  iMod (socket_address_group_own_alloc_subseteq_pre _ (to_singletons A)
+                                                      (to_singletons A)
+         with "Hauth") as
+      "[Hauth HownA]"; [done|].
+  iDestruct (socket_address_group_own_big_sepS with "HownA") as "#HownAS".
+  iMod (messages_ctx_init (to_singletons A) _ _ _ _ with "HownAS Hobserved_send Hobserved_receive" ) as (γms) "[Hms HB]".
+  iMod (steps_init 1) as (γsteps) "[Hsteps _]".
+  iMod (roles_init ((simple_live_roles st) : gset $ fmrole simple_fair_model)) as (γlive) "[Hlivefull Hlivefrag]".
+  iMod (roles_init ((all_roles ∖ simple_live_roles st) : gset $ fmrole simple_fair_model))
+    as (γdead) "[Hdeadfull Hdeadfrag]".
+  iMod (alloc_evs_init lbls) as (γalevs) "[Halobctx Halobs]".
+  iMod (sendreceive_evs_init (to_singletons obs_send_sas)) as
+      (γsendevs) "[Hsendevsctx Hsendevs]".
+  iMod (sendreceive_evs_init (to_singletons obs_rec_sas)) as
+    (γreceiveevs) "[Hreceiveevsctx Hreceiveevs]".
+  iMod (model_init (model_draft.Start:(fair_model_to_model simple_fair_model).(mstate))) as (γm) "[Hmfull Hmfrag]".
+  set (dg :=
+         {|
+           aneris_node_gnames_name := γmp;
+           aneris_si_name := γsi;
+           aneris_socket_address_group_name := γC;
+           aneris_unallocated_socket_address_groups_name := γsif;
+           aneris_freeips_name := γips;
+           aneris_freeports_name := γpiu;
+           aneris_messages_name := γms;
+           aneris_model_name := γm;
+           aneris_live_roles_name := γlive;
+           aneris_dead_roles_name := γdead;
+           aneris_steps_name := γsteps;
+           aneris_allocEVS_name := γalevs;
+           aneris_sendonEVS_name := γsendevs;
+           aneris_receiveonEVS_name := γreceiveevs;
+           aneris_observed_send_name := γobserved_send;
+           aneris_observed_recv_name := γobserved_receive;
+         |}).
+  iMod (Hwp dg) as "Hwp".
+  iMod (node_ctx_init ∅ ∅) as (γn) "[Hh Hs]".
+  iMod (node_gnames_alloc γn _ ip with "[$]") as "[Hmp #Hγn]"; [done|].
+  iAssert (is_node ip) as "Hn".
+  { iExists _. eauto. }
+  iExists (λ ex atr,
+      (⌜simple_valid_state_evolution ex atr⌝ ∗
+       aneris_events_state_interp ex ∗
+       aneris_state_interp
+         (trace_last ex).2
+         (trace_messages_history ex) ∗
+       thread_live_roles_interp (trace_last ex).1 (trace_last atr) ∗
+       steps_auth (trace_length ex)))%I.
+  iExists (map (λ '(tnew,e) v, fork_post (locale_of tnew e) v) (prefixes es))%I,
+            (fork_post)%I.
+  iSplitR; [by iApply config_wp_correct|].
+   iMod (socket_address_group_own_alloc_subseteq_pre _ (to_singletons A) (to_singletons obs_send_sas) with "Hauth")
+    as "[Hauth Hown_send]".
+   { intros x Hin. eapply elem_of_to_singletons. set_solver. }
+  iDestruct (socket_address_group_own_big_sepS with "Hown_send") as "Hown_send".
+  iMod (socket_address_group_own_alloc_subseteq_pre _ (to_singletons A) (to_singletons obs_rec_sas) with "Hauth")
+    as "[Hauth Hown_recv]".
+  { intros x Hin. eapply elem_of_to_singletons. set_solver. }
+  iAssert (live_roles_frag_own (((simple_live_roles st) : gset $ fmrole simple_fair_model) ∖ config_roles) ∗
+           live_roles_frag_own (((simple_live_roles st) : gset $ fmrole simple_fair_model) ∩ config_roles))%I with
+            "[Hlivefrag]" as "[Hlivefrag Hlivefrag_cfg]".
+  { iApply live_roles_own_split; [set_solver|].
+    by rewrite -gset_union_difference_intersection_L. }
+  iAssert (dead_roles_frag_own (((all_roles ∖ simple_live_roles st) : gset $ fmrole simple_fair_model) ∖ config_roles) ∗
+           dead_roles_frag_own (((all_roles ∖ simple_live_roles st) : gset $ fmrole simple_fair_model) ∩ config_roles))%I with
+            "[Hdeadfrag]" as "[Hdeadfrag Hdeadfrag_cfg]".
+  { iApply dead_roles_own_split; [set_solver|].
+    by rewrite -gset_union_difference_intersection_L. }
+  iDestruct (socket_address_group_own_big_sepS with "Hown_recv") as "Hown_recv".
+  iDestruct ("Hwp" with "Hunallocated [HB] Hlivefrag Hdeadfrag HIPs Hn Halobs
+            [Hsendevs Hown_send] [Hreceiveevs Hown_recv]
+            Hobserved_send Hobserved_receive") as ">Hwp".
+  { iApply (big_sepS_to_singletons with "[] HB").
+    iIntros "!>" (x) "Hx".
+    iDestruct "Hx" as (As Ar) "(?&?&[%%]&?&?)".
+    iFrame. simpl. iSplitL; [|done].
+    iExists _, _. iFrame.
+    iPureIntro.
+    rewrite H H0. rewrite !bool_decide_eq_true. admit. }
+  { iApply big_sepS_sep.
+    iSplitL "Hown_send".
+    - iApply (big_sepS_to_singletons with "[] Hown_send"); by eauto.
+    - iApply (big_sepS_to_singletons with "[] Hsendevs"); by eauto. }
+  { iApply big_sepS_sep.
+    iSplitL "Hown_recv".
+    - iApply (big_sepS_to_singletons with "[] Hown_recv"); by eauto.
+    - iApply (big_sepS_to_singletons with "[] Hreceiveevs"); by eauto. }
+  iMod (socket_address_group_own_alloc_subseteq_pre _ (to_singletons A)
+                                                    (to_singletons (obs_send_sas ∪ obs_rec_sas)) with "Hauth")
+    as "[Hauth Hown_send_recv]"; [by set_solver|].
+  rewrite to_singletons_union.
+  iPoseProof (aneris_events_state_interp_init with "[$] [$] [$] [$] [$] [$]") as "$".
+  iMod (socket_address_group_own_alloc_subseteq_pre _ (to_singletons A)
+                                                    (to_singletons A) with "Hauth")
+    as "[Hauth Hown]"; [by set_solver|].
+  iPoseProof (@aneris_state_interp_init _ _ dg IPs
+               with "Hmp [//] Hh Hs Hms [$Hauth $Hown] Hunallocated_auth Hsi HIPsCtx HPiu") as "Hinterp"; eauto.
+  { iPureIntro. apply to_singletons_fmap. intros x. rewrite /is_ne. set_solver. }
+  iModIntro.
+  iSplitR "Hwp".
+  { iSplitR.
+    { iPureIntro. split; [constructor|done]. }
+    iFrame "Hsteps".
+    (* TODO: Change definition in state interp *)
+    replace ((all_roles ∖ simple_live_roles st) ∩ config_roles) with
+      (config_roles ∖ simple_live_roles st) by set_solver.
+    rewrite /= Hmse /= dom_empty_L. by iFrame. }
+  iFrame "Hwp".
+  iIntros (ex atr c Hvalex Hstartex Hstartatr Hendex Hcontr Hstuck Htake)
+          "Hsi Hposts".
+  iDestruct "Hsi" as "(%Hvalid&_&_&Hlive&_)".
+  iApply fupd_mask_intro; [set_solver|].
+  iIntros "_".
+  iAssert (⌜locale_dead_role_disabled c (trace_last atr)⌝)%I as "%Hrole".
+  { iIntros (ℓ ζ Hmatch e Hlocale Hval).
+    iAssert (dead_role_frag_own ℓ)%I with "[Hposts]" as "H".
+    { rewrite -map_app -prefixes_from_app.
+      iDestruct (posts_of_length_drop with "Hposts") as "Hposts"; [done|].
+      destruct Hval as [v Hv].
+      iDestruct (posts_of_idx with "Hposts") as (ℓ' Hmatch') "H"; [done|done|].
+      rewrite /labels_match in Hmatch.
+      rewrite /labels_match in Hmatch'.
+      rewrite -Hmatch in Hmatch'. simplify_eq. done. }
+    simpl in *.
+    iDestruct "Hlive" as "(_&_&Hdead&Hdead')".
+    iDestruct (dead_role_auth_elem_of with "Hdead H") as %Hin.
+    iPureIntro.
+    intros Hneq. set_solver. }
+  iPureIntro.
+  pose proof Hvalid as Hvalid'.
+  destruct Hvalid as (Htrace&Hlabels&Hstate).
+  split; [done|].
+  split; [done|].
+  apply valid_state_live_tids; [done|].
+  by rewrite Hendex.
+Admitted.
+
+Theorem strong_simulation_adequacy Σ
+    `{!anerisPreG simple_fair_model Σ}
+    (s : stuckness) (e : aneris_expr) (σ : state) (st : simple_state)
+    A obs_send_sas obs_rec_sas IPs ip lbls :
+  role_enabled_locale_exists ([e], σ) st →
+  state_ms σ = mABn (state_get_n st) →
+  (∃ shA shB : socket_handle,
+      state_sockets σ =
+      {[ipA := {[shA := (sA, [])]};
+        ipB := {[shB := (sB, mABm (state_get_m st))]}]}) →
+  wp_proto IPs A lbls obs_send_sas obs_rec_sas s [e] ip st →  
+  obs_send_sas ⊆ A → obs_rec_sas ⊆ A →
+  ip ∉ IPs →
+  dom (state_ports_in_use σ) = IPs →
+  (∀ ip, ip ∈ IPs → state_ports_in_use σ !! ip = Some ∅) →
+  (∀ a, a ∈ A → ip_of_address a ∈ IPs) →
+  state_heaps σ = {[ip:=∅]} →
+  state_sockets σ = {[ip:=∅]} →
+  state_ms σ = ∅ →
+  continued_simulation_init valid_state_evolution_fairness ([e], σ) st.
+Proof.
+  intros ??? Hwp. by eapply strong_simulation_adequacy_multiple; [simpl;lia|..].
+Qed.
+
+(* TODO: Should generalise this for more languages *)
+Definition fair_network_ex (extr : extrace aneris_lang) :=
+  ∀ n, pred_at extr n (λ _ ζ, ζ ≠ Some (inr DuplicateLabel) ∧
+                              ζ ≠ Some (inr DropLabel)).
+
+Definition fair_ex (extr : extrace aneris_lang) :=
+  (∀ ζ, fair_scheduling_ex ζ extr) ∧ fair_network_ex extr.
+
+Definition live_traces_match : extrace aneris_lang → mtrace simple_fair_model → Prop :=
+  traces_match labels_match live_tids language.locale_step simple_trans.
+
+(* TODO: Clean this up - Currently just ported directly from Fairness *)
+Lemma valid_inf_system_trace_implies_traces_match
+      ex atr iex iatr progtr (auxtr : mtrace simple_fair_model) :
+  exec_trace_match ex iex progtr ->
+  exec_trace_match atr iatr auxtr ->
+  valid_inf_system_trace (continued_simulation valid_state_evolution_fairness) ex atr iex iatr ->
+  live_traces_match progtr auxtr.
+Proof.
+  revert ex atr iex iatr auxtr progtr. cofix IH.
+  intros ex atr iex iatr auxtr progtr Hem Ham Hval.
+  inversion Hval as [?? Hphi |
+                      ex' atr' c [? σ'] δ' iex' iatr' oζ ℓ Hphi [=] ? Hinf];
+    simplify_eq.
+  - inversion Hem; inversion Ham. econstructor.
+    apply continued_simulation_rel in Hphi as (Hsteps&Hmatch&Hlive).
+    by simplify_eq.
+  - inversion Hem; inversion Ham. subst.
+    pose proof (valid_inf_system_trace_inv _ _ _ _ _ Hinf) as Hphi'.
+    apply continued_simulation_rel in Hphi as (Hmatch&Hsteps&Hlive).
+    apply continued_simulation_rel in Hphi' as (Hsteps'&Hmatch'&Hlive').
+    econstructor.
+    + eauto.
+    + eauto.
+    + match goal with
+      | [H: exec_trace_match _ iex' _ |- _] => inversion H; clear H; simplify_eq
+      end; done.
+    + match goal with
+      | [H: exec_trace_match _ iatr' _ |- _] => inversion H; clear H; simplify_eq
+      end.
+      * inversion Hsteps'; simplify_eq.
+        rewrite /trace_ends_in in H3. rewrite H3. done.
+      * simpl. inversion Hsteps'; simplify_eq.
+        rewrite /trace_ends_in in H4. rewrite H4. done.
+    + eapply IH; eauto.
+Qed.
+
+Definition extrace_matching_mtrace_exists st extr :=
+   ∃ mtr, trfirst mtr = st ∧ live_traces_match extr mtr.
+
+Lemma continued_simulation_traces_match extr st :
+  extrace_valid extr →
+  continued_simulation valid_state_evolution_fairness
+                       {tr[trfirst extr]} {tr[st]} →
+  extrace_matching_mtrace_exists st extr.
+Proof.
+  intros Hvalid Hsim.
+  assert (∃ iatr,
+             valid_inf_system_trace
+               (continued_simulation valid_state_evolution_fairness)
+               (trace_singleton (trfirst extr))
+               (trace_singleton (st))
+               (from_trace extr)
+               iatr) as [iatr Hiatr].
+  { eexists _. eapply produced_inf_aux_trace_valid_inf. econstructor.
+    Unshelve.
+    - done.
+    - eapply from_trace_preserves_validity; eauto; first econstructor. }
+  eexists _.
+  split; last first.
+  { eapply (valid_inf_system_trace_implies_traces_match); eauto.
+    - by apply from_trace_spec.
+    - by apply to_trace_spec. }
+  destruct iatr; [done|by destruct x].
+Qed.
+
+Definition matching_mtrace_exists c st :=
+  extrace_property c (extrace_matching_mtrace_exists st).
+
+(** A continued simulation exists between some initial configuration [c]
+    and the initial state [init_state] of a fair model. *)
+Definition live_simulation (c : cfg aneris_lang) (st : simple_state) :=
+  continued_simulation_init valid_state_evolution_fairness c st.
+
+Lemma continued_simulation_traces_match_init c st :
+  live_simulation c st → matching_mtrace_exists c st.
+Proof.
+  intros Hsim extr <- Hvalid.
+  apply (continued_simulation_traces_match) in Hsim
+      as (mtr & Hmtr & Hmatch); [by eexists _|done].
+Qed.
+
+Lemma traces_match_valid_preserved extr mtr :
+  live_traces_match extr mtr → mtrace_valid mtr.
+Proof.
+  revert extr mtr. pcofix CH. intros extr mtr Hmatch.
+  inversion Hmatch; first by (pfold; constructor).
+  pfold. constructor =>//.
+  specialize (CH _ _ H3). by right.
+Qed.
+
+Lemma traces_match_fairness_preserved extr mtr :
+  live_traces_match extr mtr → fair_ex extr → mtrace_fair mtr.
+Proof.
+  rewrite /fair_ex /mtrace_fair.
+  intros Hmatch [Hfairex_scheduling Hfairex_network].
+  assert (mtrace_valid mtr) as Hvalid.
+  { by eapply traces_match_valid_preserved. }
+  split.
+  - intros ℓ.
+    assert (∃ ζ, labels_match ζ ℓ) as [ζ Hlabel].
+    { exists (simple_label_locale ℓ). destruct ℓ; done. }
+    specialize (Hfairex_scheduling ζ).
+    eapply traces_match_traces_implies; [done| | |done].
+    + intros s1 s2 oℓ1 oℓ2 Hlive HRℓ Henabled.
+      simpl in *. simplify_eq.
+      apply Hlive in Hlabel.
+      by apply Hlabel.
+    + intros s1 s2 oℓ1 oℓ2 Hlive HRℓ [Henabled|Henabled]; simpl in *.
+      * left. intros Henabled'. apply Henabled.
+        apply Hlive in Hlabel. by apply Hlabel.
+      * right. rewrite Henabled in HRℓ. destruct oℓ2; [|done].
+        simplify_eq. rewrite Hlabel. by rewrite HRℓ.
+  - intros n. rewrite /pred_at.
+    specialize (Hfairex_network n). rewrite /pred_at in Hfairex_network.
+    destruct (after n extr) eqn:Heqn; [|done].
+    apply traces_match_flip in Hmatch; [|done..].
+    eapply (traces_match_after) in Hmatch as (mtr' & Hmtreq & Hmatch); [|done].
+    rewrite Hmtreq.
+    destruct t; inversion Hmatch; simplify_eq; [done|].
+    destruct Hfairex_network as [Hdup Hdrop].
+    split.
+    + rewrite H2. intros Heq. apply Hdup. simplify_eq.
+      rewrite /locale_simple_label in Heq.
+      repeat case_match; simplify_eq.
+    + rewrite H2. intros Heq. apply Hdrop. simplify_eq.
+      rewrite /locale_simple_label in Heq.
+      repeat case_match; simplify_eq.
+Qed.
+
+Lemma traces_match_termination_preserved extr mtr :
+  live_traces_match extr mtr → terminating_trace mtr → terminating_trace extr.
+Proof. intros Hmatch [n Hmtr]. exists n. by eapply traces_match_after_None. Qed.
+
+Definition extrace_fairly_terminating (extr : extrace aneris_lang) :=
+  fair_ex extr → terminating_trace extr.
+
+Lemma traces_match_fair_termination_preserved extr mtr :
+  initial_reachable mtr →
+  live_traces_match extr mtr →
+  extrace_fairly_terminating extr.
+Proof.
+  intros Hinitial Hsim Hfair.
+  eapply traces_match_termination_preserved; [done|].
+  eapply fair_terminating_traces_terminate;
+    [done|by eapply traces_match_valid_preserved|
+      by eapply traces_match_fairness_preserved].
+Qed.
+
+Definition init_state := model_draft.Start.
+
+Lemma initial_reachable_start mtr :
+  tr_starts_in mtr init_state → initial_reachable mtr.
+Proof.
+  rewrite /tr_starts_in. intros Hstart.
+  (* TODO: Clean this up *)
+  rewrite /initial_reachable. rewrite /initial_reachable in Hstart.
+  destruct mtr; rewrite /pred_at; rewrite /pred_at in Hstart; simpl in *;
+                by simplify_eq.
+Qed.
+
+Definition fairly_terminating (c : cfg aneris_lang) :=
+  extrace_property c extrace_fairly_terminating.
+
+Lemma traces_match_fair_termination_preserved_init c :
+  matching_mtrace_exists c init_state → fairly_terminating c.
+Proof.
+  intros Hmatches.
+  eapply extrace_property_impl; [done|].
+  intros extr Hstart Hvalid (mtr & Hstart' & Hmtr) Hfair.
+  eapply traces_match_fair_termination_preserved; [|done..].
+  by apply initial_reachable_start.
+Qed.
+
+Theorem continued_simulation_fair_termination c :
+  live_simulation c init_state → fairly_terminating c.
+Proof.
+  intros ?.
+  by apply traces_match_fair_termination_preserved_init,
+    continued_simulation_traces_match_init.
+Qed.
+
+Theorem simulation_adequacy_fair_termination_multiple Σ
+    `{!anerisPreG simple_fair_model Σ}
+    (s : stuckness) (es : list aneris_expr) (σ : state)
+    A obs_send_sas obs_rec_sas IPs ip lbls :
+  length es ≥ 1 →
+  role_enabled_locale_exists (es, σ) init_state →
+  state_ms σ = mABn (state_get_n init_state) →
+  (∃ shA shB : socket_handle,
+      state_sockets σ =
+      {[ipA := {[shA := (sA, [])]};
+        ipB := {[shB := (sB, mABm (state_get_m init_state))]}]}) →
+  wp_proto IPs A lbls obs_send_sas obs_rec_sas s es ip init_state →
+  obs_send_sas ⊆ A → obs_rec_sas ⊆ A →
+  ip ∉ IPs →
+  dom (state_ports_in_use σ) = IPs →
+  (∀ ip, ip ∈ IPs → state_ports_in_use σ !! ip = Some ∅) →
+  (∀ a, a ∈ A → ip_of_address a ∈ IPs) →
+  state_heaps σ = {[ip:=∅]} →
+  state_sockets σ = {[ip:=∅]} →
+  state_ms σ = ∅ →
+  fairly_terminating (es,σ).
+Proof.
+  intros. by eapply continued_simulation_fair_termination,
+            strong_simulation_adequacy_multiple.
+Qed.
