fairneris/examples/retransmit_model.v
@@ -1,0 +1,490 @@
+From trillium.prelude Require Export finitary quantifiers sigma classical_instances.
+From Paco Require Import paco1 paco2 pacotac.
+From fairneris Require Export trace_utils fairness.
+From fairneris.aneris_lang Require Import ast network.
+
+Import derived_laws_later.bi.
+
+Lemma prefix_trans {A} (l1 l2 l3 : list A) :
+  l1 `prefix_of` l2 → l2 `prefix_of` l3 → l1 `prefix_of` l3.
+Proof. intros [l1' ->] [l2' ->]. by do 2 apply prefix_app_r. Qed.
+
+Lemma suffix_trans {A} (l1 l2 l3 : list A) :
+  l1 `suffix_of` l2 → l2 `suffix_of` l3 → l1 `suffix_of` l3.
+Proof. intros [l1' ->] [l2' ->]. by do 2 apply suffix_app_r. Qed.
+
+(** The retransmit model states *)
+Inductive retransmit_base_state :=
+| Start
+| Received.
+
+Definition retransmit_state : Set :=
+  retransmit_base_state * message_multi_soup * gmap socket_address (list message).
+
+#[global] Instance simple_state_eqdec : EqDecision retransmit_state.
+Proof. intros ??. apply make_decision. Qed.
+#[global] Instance simple_state_inhabited : Inhabited retransmit_state.
+Proof. exact (populate (Start,∅,∅)). Qed.
+
+Inductive retransmit_node_role := Arole | Brole.
+(* Inductive retransmit_network_role := *)
+(* | Ndup *)
+(* | Ndrop *)
+(* | Ndeliver. *)
+Definition retransmit_network_role : Set := unit.
+Definition retransmit_role : Set :=
+  retransmit_node_role + retransmit_network_role.
+
+Definition retransmit_node_action : Set := option message.
+Definition retransmit_network_action : Set := option message.
+Definition retransmit_action : Set :=
+  retransmit_node_action + retransmit_network_action.
+
+Definition retransmit_node_label : Set :=
+  retransmit_node_role * retransmit_node_action.
+Definition retransmit_network_label : Set :=
+  retransmit_network_role * retransmit_network_action.
+Definition retransmit_label : Set :=
+  retransmit_node_label + retransmit_network_label.
+
+Definition label_role (l : retransmit_label) : retransmit_role :=
+  sum_map fst fst l.
+Definition label_action (l : retransmit_label) : retransmit_action :=
+  sum_map snd snd l.
+
+#[global] Instance retransmit_node_role_eqdec : EqDecision retransmit_node_role.
+Proof. intros ??. apply make_decision. Qed.
+#[global] Instance retransmit_node_role_inhabited : Inhabited retransmit_node_role.
+Proof. exact (populate (Arole)). Qed.
+#[global] Instance retransmit_node_role_countable : Countable retransmit_node_role.
+Proof.
+  refine ({|
+             encode s := match s with
+                         | Arole => 1
+                         | Brole => 2
+                         end;
+             decode n := match n with
+                         | 1 => Some Arole
+                         | 2 => Some Brole
+                         | _ => None
+                         end;
+         |})%positive.
+  by intros [|].
+Qed.
+
+#[global] Instance retransmit_role_eqdec : EqDecision retransmit_role.
+Proof. intros ??. apply make_decision. Qed.
+#[global] Instance retransmit_role_inhabited : Inhabited retransmit_role.
+Proof. exact (populate (inl Arole)). Qed.
+#[global] Instance retransmit_role_countable : Countable retransmit_role.
+Proof.
+  refine ({|
+             encode s := match s with
+                         | inl Arole => 1
+                         | inl Brole => 2
+                         | inr () => 3
+                         end;
+             decode n := match n with
+                         | 1 => Some $ inl Arole
+                         | 2 => Some $ inl Brole
+                         | 3 => Some $ inr ()
+                         | _ => None
+                         end;
+         |})%positive.
+  by intros [[]|[]].
+Qed.
+
+Definition saA : socket_address := SocketAddressInet "0.0.0.0" 80.
+Definition saB : socket_address := SocketAddressInet "0.0.0.1" 80.
+Definition mAB : message := mkMessage saA saB "Hello".
+
+Inductive retransmit_trans : retransmit_state → retransmit_label → retransmit_state → Prop :=
+| A_Send st ms bs :
+  retransmit_trans (st, ms, bs)
+                   (inl $ (Arole, Some mAB))
+                   (st, ms ⊎ {[+ mAB +]}, bs)
+| N_Duplicate st ms bs msg :
+  msg ∈ ms →
+  retransmit_trans (st, ms, bs)
+                   (inr ((),None))
+                   (st, ms ⊎ {[+ msg +]}, bs)
+| N_Drop st ms bs msg :
+  msg ∈ ms →
+  retransmit_trans (st, ms, bs)
+                   (inr ((), None))
+                   (st, ms ∖ {[+ msg +]}, bs)
+| N_Deliver st ms ms' bs msg :
+  msg ∈ ms →
+  bs !!! m_destination msg = ms' →
+  retransmit_trans (st, ms, bs)
+                   (inr ((), Some msg))
+                   (st, ms ∖ {[+ msg +]}, <[m_destination msg := msg::ms']>bs)
+| B_RecvFail ms bs :
+  bs !!! saB = [] →
+  retransmit_trans (Start, ms, bs)
+                   (inl $ (Brole, None))
+                   (Start, ms, bs)
+| B_RecvSucc ms bs msg ms' :
+  bs !!! saB = ms'++[msg] →
+  retransmit_trans (Start, ms, bs)
+                   (inl $ (Brole, None))
+                   (Received, ms, <[saB := ms']>bs).
+
+Definition send_filter msg : retransmit_state → retransmit_label → Prop :=
+  λ _ l, label_action l = inl $ Some msg.
+Instance send_filter_decision msg st l : Decision (send_filter msg st l).
+Proof. apply make_decision. Qed.
+
+Definition deliver_filter msg : retransmit_state → retransmit_label → Prop :=
+  λ _ l, l = inr ((),Some msg).
+Instance deliver_filter_decision msg st l : Decision (deliver_filter msg st l).
+Proof. apply make_decision. Qed.
+
+Class Monotone (f : nat → nat) :=
+  { mono_incr : ∀ n m, n ≤ m → f n ≤ f m; }.
+
+Definition count_sends (msg : message) tr : nat :=
+  count_labels (trace_filter (send_filter msg) tr).
+
+Definition count_delivers (msg : message) tr : nat :=
+  count_labels (trace_filter (deliver_filter msg) tr).
+
+Notation mtrace := (trace retransmit_state retransmit_label).
+
+Definition retransmit_network_fair_delivery (tr : mtrace) : Prop :=
+  ∃ (f1 f2 : nat → nat) `(Monotone f1) `(Monotone f2),
+    ∀ msg n,
+      let sends := count_sends msg (trace_take n tr) in
+      let delivers := count_delivers msg (trace_take n tr) in
+      f1 delivers ≤ sends ≤ f2 delivers.
+
+(* TODO: This computation is a bit odd *)
+(* Definition retransmit_live_roles (s : retransmit_state) : gset retransmit_role := *)
+(*   {[inl Arole]} ∪ *)
+(*   (if decide (s.1.2 = (∅:gmultiset _)) then ∅ *)
+(*    else {[inr Ndup;inr Ndrop;inr Ndeliver]}) ∪ *)
+(*   (match s.1.1 with Start => {[inl Brole]} | _ => ∅ end). *)
+Definition retransmit_live_roles (s : retransmit_state) : gset retransmit_node_role :=
+  {[Arole]} ∪
+  (match s.1.1 with Start => {[Brole]} | _ => ∅ end).
+
+(* TODO: This should be generalised, and lifted to multiple roles *)
+Definition retransmit_terminating_role (ρ : retransmit_node_role) (tr : mtrace) : Prop :=
+  ∃ n, after n tr = None ∨
+       pred_at tr n (λ st _, ρ ∉ retransmit_live_roles st).
+
+Definition retransmit_role_enabled_model (ρ : retransmit_node_role) (s : retransmit_state) : Prop :=
+  ρ ∈ retransmit_live_roles s.
+
+Definition retransmit_fair_scheduling_mtr (ρ : retransmit_node_role) : mtrace → Prop :=
+  trace_implies (λ δ _, retransmit_role_enabled_model ρ δ)
+                (λ δ ℓ, ¬ retransmit_role_enabled_model ρ δ ∨
+                          option_map label_role ℓ = Some (inl ρ)).
+
+Lemma retransmit_fair_scheduling_mtr_after ℓ tr tr' k :
+  after k tr = Some tr' →
+  retransmit_fair_scheduling_mtr ℓ tr → retransmit_fair_scheduling_mtr ℓ tr'.
+Proof. apply trace_implies_after. Qed.
+
+Definition retransmit_fair_scheduling (mtr : mtrace) : Prop :=
+  ∀ ρ, retransmit_fair_scheduling_mtr ρ mtr.
+
+Lemma retransmit_fair_scheduling_after tr tr' k :
+  after k tr = Some tr' →
+  retransmit_fair_scheduling tr → retransmit_fair_scheduling tr'.
+Proof.
+  intros Hafter Hfair ℓ. specialize (Hfair ℓ).
+  by eapply retransmit_fair_scheduling_mtr_after.
+Qed.
+
+Definition mtrace_fair (mtr : mtrace) : Prop :=
+  retransmit_fair_scheduling mtr ∧ retransmit_network_fair_delivery mtr.
+
+Inductive mtrace_valid_ind (mtrace_valid_coind: mtrace → Prop) :
+  mtrace → Prop :=
+| mtrace_valid_singleton δ: mtrace_valid_ind _ ⟨δ⟩
+| mtrace_valid_cons δ ℓ tr:
+  retransmit_trans δ ℓ (trfirst tr) →
+  mtrace_valid_coind tr →
+  mtrace_valid_ind _ (δ -[ℓ]-> tr).
+Definition mtrace_valid := paco1 mtrace_valid_ind bot1.
+
+Lemma mtrace_valid_mono :
+  monotone1 mtrace_valid_ind.
+Proof.
+  unfold monotone1. intros x0 r r' IN LE.
+  induction IN; try (econstructor; eauto; done).
+Qed.
+Hint Resolve mtrace_valid_mono : paco.
+
+Lemma mtrace_valid_after (mtr mtr' : mtrace) k :
+  after k mtr = Some mtr' → mtrace_valid mtr → mtrace_valid mtr'.
+Proof.
+  revert mtr mtr'.
+  induction k; intros mtr mtr' Hafter Hvalid.
+  { destruct mtr'; simpl in *; by simplify_eq. }
+  punfold Hvalid.
+  inversion Hvalid as [|??? Htrans Hval']; simplify_eq.
+  eapply IHk; [done|].
+  by inversion Hval'.
+Qed.
+
+Lemma retransmit_trace_delivers_0 mtr n :
+  (∀ n, pred_at mtr n (λ _ l, l ≠ Some $ inr ((), Some mAB))) →
+  count_delivers mAB (trace_take n mtr) = 0.
+Proof.
+  revert mtr.
+  induction n as [|n IHn]; intros mtr Hpred=> /=; [by destruct mtr|].
+  destruct mtr as [|s l mtr]; [done|]. rewrite /count_delivers=> /=.
+  case_bool_decide as Hb.
+  - specialize (Hpred 0). rewrite pred_at_0 in Hpred.
+    rewrite /deliver_filter in Hb. by simplify_eq.
+  - apply IHn. intros n'. specialize (Hpred (S n')).
+    by rewrite pred_at_S in Hpred.
+Qed.
+
+Lemma A_always_live (mtr : mtrace) n :
+  infinite_trace mtr →
+  pred_at mtr n (λ s _, retransmit_role_enabled_model (Arole) s).
+Proof.
+  rewrite /pred_at /retransmit_role_enabled_model. intros [mtr' ->].
+  by destruct mtr'; set_solver.
+Qed.
+
+Lemma retransmit_fair_traces_eventually_A mtr :
+  infinite_trace mtr → retransmit_fair_scheduling mtr →
+  ∃ n, pred_at mtr n (λ _ ℓ, option_map label_role ℓ = Some $ inl Arole).
+Proof.
+  intros Hinf Hfair.
+  pose proof (A_always_live mtr 0 Hinf) as HA.
+  apply Hfair in HA as [m HA]. apply pred_at_or in HA as [HA|HA]; [|by exists m].
+  pose proof (A_always_live mtr m Hinf) as HA'. by apply pred_at_neg in HA.
+Qed.
+
+Lemma retransmit_fair_traces_eventually_mAB mtr :
+  infinite_trace mtr → mtrace_valid mtr → retransmit_fair_scheduling mtr →
+  ∃ n, pred_at mtr n (λ st l, option_map label_action l = Some $ inl $ Some mAB).
+Proof.
+  intros Hinf Hvalid Hfair.
+  pose proof (retransmit_fair_traces_eventually_A mtr) as [m HA]; [done..|].
+  exists m. specialize (Hinf m) as [mtr' Hafter].
+  eapply mtrace_valid_after in Hvalid; [|done].
+  rewrite /pred_at Hafter in HA. rewrite /pred_at Hafter.
+  destruct mtr'; [done|]. destruct ℓ; [|done]. destruct r. simpl in *.
+  simplify_eq. pinversion Hvalid. inversion H1. by simplify_eq.
+Qed.
+
+(* TODO: This can possibly be generalised *)
+Lemma count_sends_pred_at n tr :
+  pred_at tr n (λ _ l, option_map label_action l = Some $ inl $ Some mAB) →
+  0 < count_sends mAB (trace_take (S n) tr).
+Proof.
+  revert tr. induction n as [|n IHn]=> /=; intros tr Hpred_at.
+  { rewrite /pred_at in Hpred_at. destruct tr; [done|].
+    rewrite /count_sends=> /=.
+    case_bool_decide as Hb; [by simpl; lia|].
+    destruct ℓ; [|done]. rewrite /send_filter in Hb.
+    destruct r. simpl in *. simplify_eq. }
+  destruct tr; [done|]. rewrite /count_sends=> /=.
+  case_bool_decide as Hb; [simpl; lia|by apply IHn].
+Qed.
+
+(* Any fair infinite trace grow the number of sends indefinitely *)
+Lemma retransmit_trace_sends_grows mtr x :
+  infinite_trace mtr → mtrace_valid mtr → retransmit_fair_scheduling mtr →
+  ∃ n, x < count_sends mAB (trace_take n mtr).
+Proof.
+  intros Hafter Hvalid Hfair.
+  induction x as [|x IHx].
+  { pose proof (retransmit_fair_traces_eventually_mAB) as [n Hn]; [done..|].
+    exists (S n). by eapply count_sends_pred_at. }
+  destruct IHx as [n Hn].
+  apply (infinite_trace_after' n) in Hafter as (mtr' & Hmtr' & Hafter).
+  apply (mtrace_valid_after _ mtr' n) in Hvalid; [|done].
+  apply (retransmit_fair_scheduling_after _ mtr' n) in Hfair; [|done].
+  pose proof (retransmit_fair_traces_eventually_mAB) as [m Hm]; [done..|].
+  assert (0 < count_sends mAB (trace_take (S m) mtr')) as Hcount.
+  { by eapply count_sends_pred_at. }
+  exists (n+(S m)).
+  rewrite /count_sends. rewrite /count_sends in Hcount.
+  rewrite /count_sends in Hn. rewrite (count_labels_sum _ _ _ _ mtr'); [lia|done].
+Qed.
+
+(* Any fair trace eventually delivers a message *)
+Lemma retransmit_fair_trace_eventually_Ndeliver mtr :
+  infinite_trace mtr → mtrace_valid mtr → mtrace_fair mtr →
+  ∃ n, pred_at mtr n (λ st l, l = Some $ inr ((),Some mAB)).
+Proof.
+  intros Hafter Hvalid Hfair.
+  assert ((∃ n, pred_at mtr n (λ _ l, l = Some (inr ((), Some mAB)))) ∨
+            ¬ ∃ n, pred_at mtr n (λ _ l, l = Some (inr ((), Some mAB))))
+    as Hpred_at.
+  { apply ExcludedMiddle. }
+  destruct Hpred_at as [Hpred_at|Hpred_at]; [done|].
+  assert False; [|done].
+  destruct Hfair as [Hfair_sched Hfair_network].
+  destruct Hfair_network as (f1&f2&?&?&Hfair_network).
+  pose proof (retransmit_trace_sends_grows mtr (f2 0)) as [m Hm]; [done..|].
+  specialize (Hfair_network mAB m).
+  destruct Hfair_network as [_ Hfair_network2].
+  rewrite retransmit_trace_delivers_0 in Hfair_network2; [lia|].
+  intros n. apply pred_at_neg; [done|].
+  by eapply not_exists_forall_not in Hpred_at.
+Qed.
+
+Lemma Ndeliver_adds_to_buffer msg s bs (mtr:mtrace) :
+  mtrace_valid (s -[inr ((),Some msg)]-> mtr) →
+  (trfirst (s -[inr ((),Some msg)]-> mtr)).2 !!! m_destination msg = bs →
+  (trfirst mtr).2 !!! (m_destination msg) = msg :: bs.
+Proof.
+  intros Hvalid <-. pinversion Hvalid; simplify_eq. inversion H1; simplify_eq.
+  by rewrite lookup_total_insert.
+Qed.
+
+Lemma retransmit_fair_trace_buffer_grows mtr n mtr' :
+  mtrace_valid mtr →
+  (∀ m, m < n → pred_at mtr m
+                  (λ _ l, option_map label_role l ≠ Some $ inl Brole)) →
+  after n mtr = Some mtr' →
+  suffix ((trfirst mtr).2 !!! saB) ((trfirst mtr').2 !!! saB).
+Proof.
+  revert mtr. induction n as [|n IHn]; intros mtr Hvalid Halways Hafter.
+  { simpl in *. by simplify_eq. }
+  destruct mtr as [|s l mtr]; [done|].
+  eapply suffix_trans; last first.
+  { apply IHn; [| |done].
+    { by eapply (mtrace_valid_after _ mtr 1); [|done]. }
+    intros m Hlt. specialize (Halways (S m)). rewrite pred_at_S in Halways.
+    apply Halways. lia. }
+  punfold Hvalid. inversion Hvalid. simplify_eq.
+  inversion H1; simplify_eq; try set_solver.
+  - destruct (decide (m_destination msg = saB)) as [->|Hneq].
+    + rewrite lookup_total_insert. apply suffix_cons_r. set_solver.
+    + by rewrite lookup_total_insert_ne.
+  - assert (0 < S n) as Hlt by lia.
+    specialize (Halways 0 Hlt). rewrite pred_at_0 in Halways. simplify_eq.
+Qed.
+
+
+(* TODO: Could use more polish. Might simplify proof as well *)
+(* Any fair trace eventually ends in the receive state *)
+Lemma retransmit_fair_trace_eventually_Received mtr :
+  (trfirst mtr).1.1 = Start →
+  infinite_trace mtr → mtrace_valid mtr → mtrace_fair mtr →
+  ∃ n, pred_at mtr n (λ st _, st.1.1 = Received).
+Proof.
+  intros Htrfirst Hafter Hvalid Hfair.
+  pose proof (retransmit_fair_trace_eventually_Ndeliver) as [n Hn]; [done..|].
+  rewrite /pred_at in Hn.
+  apply (infinite_trace_after' n) in Hafter as [mtr' [Hmtr' Hafter]].
+  destruct Hfair as [Hfair1 Hfair2].
+  assert (retransmit_fair_scheduling mtr') as Hfair1'.
+  { by eapply retransmit_fair_scheduling_after. }
+  rewrite Hmtr' in Hn. destruct mtr' as [mtr'|]; [done|].
+  simplify_eq. rewrite /retransmit_fair_scheduling in Hfair1'.
+  assert ((pred_at (s -[ inr ((), Some mAB) ]-> mtr') 0
+                   (λ δ _, retransmit_role_enabled_model (Brole) δ)) ∨
+            ¬ pred_at (s -[ inr ((), Some mAB) ]-> mtr') 0
+                   (λ δ _, retransmit_role_enabled_model (Brole) δ)) as Hrole.
+  { eapply ExcludedMiddle. }
+  destruct Hrole as [Hrole|Hrole]; last first.
+  { apply pred_at_neg in Hrole; [|done]. rewrite /pred_at in Hrole.
+    exists n. rewrite /pred_at. rewrite Hmtr'.
+    rewrite /retransmit_role_enabled_model /retransmit_live_roles in Hrole.
+    destruct s as [[[]]]; [by set_solver|done]. }
+  apply Hfair1' in Hrole as [m Hm].
+  apply pred_at_or in Hm as [Hm|Hm].
+  { exists (n+m). rewrite pred_at_sum Hmtr'. eapply pred_at_impl; [|done].
+    intros [[[]]] l Hsl; [|done].
+    rewrite /retransmit_role_enabled_model /retransmit_live_roles in Hsl.
+    set_solver. }
+  assert (∃ bs, (trfirst (s -[ inr ((), Some mAB) ]-> mtr')).2 !!!
+                  m_destination mAB = bs) as [bs Hbs].
+  { by eexists _. }
+  assert (after (S n) mtr = Some mtr') as Hmtr'2.
+  { replace (S n) with (n + 1) by lia. rewrite after_sum'. by rewrite Hmtr'. }
+  apply Ndeliver_adds_to_buffer in Hbs; [|by eapply mtrace_valid_after].
+  destruct m as [|m]; [done|]. rewrite pred_at_S in Hm.
+  pose proof (trace_eventually_until mtr') as [n' [Hn' Hn'']]; [by exists m|].
+  exists (n+(S $ S n')).
+  rewrite pred_at_sum Hmtr' pred_at_S.
+  assert (pred_at mtr' n'
+                  (λ s _, suffix ((trfirst mtr').2 !!! saB) (s.2 !!! saB)))
+    as H.
+  { assert (∃ mtr'', after n' mtr' = Some mtr'') as H.
+    { apply (infinite_trace_after' (S n')) in Hafter as [mtr'' [Hmtr'' _]].
+      simpl in *. by eauto. }
+    destruct H as [mtr'' Hmtr''].
+    eapply (retransmit_fair_trace_buffer_grows _ _ mtr'') in Hn'' as Hbs';
+      [|by eapply mtrace_valid_after|done].
+    rewrite /pred_at Hmtr''. by destruct mtr''. }
+  replace (S n') with (n' + 1) by lia.
+  rewrite pred_at_sum. rewrite /pred_at in H. rewrite /pred_at in Hn'.
+  destruct (after n' mtr') as [mtr''|] eqn:Heqn; [|done].
+  assert (mtrace_valid mtr'') as Hvalid'.
+  { eapply mtrace_valid_after; [done|]. by eapply mtrace_valid_after. }
+  destruct mtr''; [naive_solver|].
+  rewrite pred_at_S /pred_at. rewrite Hbs in H.
+  inversion Hn'.
+  assert (label_role ℓ = inl Brole) as Heq.
+  { destruct ℓ; try naive_solver. }
+  destruct ℓ; simpl in *; simplify_eq. destruct r; simpl in *; simplify_eq.
+  punfold Hvalid'. inversion Hvalid'. simplify_eq.
+  inversion H2.
+  + destruct s0 as [[]]. simplify_eq. simpl in *.
+    destruct H as [? H]. rewrite H in H5. apply app_eq_nil in H5. set_solver.
+  + destruct mtr''=> /=; simpl in *; simplify_eq; set_solver.
+Qed.
+
+(* A trace starting in the receive role has partially terminated for the Brole *)
+Lemma retransmit_fair_traces_terminate_aux mtr :
+  (trfirst mtr).1.1 = Received → retransmit_terminating_role (Brole) mtr.
+Proof.
+  intros Htrfirst.
+  exists 0. rewrite /pred_at=> /=.
+  destruct mtr as [[[]]|[[]] l mtr];
+    simpl in *; simplify_eq; rewrite /retransmit_live_roles;
+    set_solver.
+Qed.
+
+(* Any fair trace terminates on role B *)
+Lemma retransmit_fair_traces_terminate mtr :
+  (trfirst mtr).1.1 = Start → mtrace_valid mtr → mtrace_fair mtr →
+  retransmit_terminating_role (Brole) mtr.
+Proof.
+  intros ???.
+  assert (infinite_trace mtr ∨ ¬ infinite_trace mtr) as [Hafter|Hafter];
+    [by apply ExcludedMiddle| |]; last first.
+  { apply not_forall_exists_not in Hafter as [n Hafter].
+    destruct (after n mtr) eqn:Heqn; [by naive_solver|].
+    exists n. by left. }
+  assert (∃ n, pred_at mtr n (λ st _, st.1.1 = Received)) as [n Hn].
+  { by apply retransmit_fair_trace_eventually_Received. }
+  rewrite /pred_at in Hn.
+  assert (∃ mtr', after n mtr = Some mtr') as [mtr' Hmtr'].
+  { destruct (after n mtr) as [mtr'|]; [|done]. by exists mtr'. }
+  rewrite Hmtr' in Hn.
+  assert ((trfirst mtr').1.1 = Received); [by destruct mtr'|].
+  assert (retransmit_terminating_role (Brole) mtr') as [m Hterminates];
+    [by apply retransmit_fair_traces_terminate_aux|].
+  exists (m+n). by rewrite pred_at_sum' after_sum Hmtr'.
+Qed.
+
+(* TODO: This is likely not needed. *)
+Lemma retransmit_live_spec_holds s ρ α s' :
+  retransmit_trans s (inl (ρ,α)) s' → ρ ∈ retransmit_live_roles s.
+Proof. inversion 1; set_solver. Qed.
+
+Definition retransmit_fair_model : FairModel.
+Proof.
+  refine({|
+            fmstate := retransmit_state;
+            fmrole := retransmit_node_role;
+            fmaction := retransmit_node_action;
+            fmconfig := retransmit_network_label;
+            fmtrans := retransmit_trans;
+            fmfairness := retransmit_network_fair_delivery;
+            live_roles := retransmit_live_roles;
+            fm_live_spec := retransmit_live_spec_holds;
+          |}).
+Defined.
