fairneris/fairness.v
@@ -1,0 +1,174 @@
+From stdpp Require Import option.
+From Paco Require Import paco1 paco2 pacotac.
+From trillium.fairness Require Export inftraces.
+From fairneris Require Export trace_utils.
+
+Record FairModel : Type := {
+  fmstate: Type;
+  fmstate_eqdec: EqDecision fmstate;
+  fmstate_inhabited: Inhabited fmstate;
+
+  fmrole: Type;
+  fmaction: Type;
+  fmconfig: Type;
+  fmrole_eqdec: EqDecision fmrole;
+  fmrole_countable: Countable fmrole;
+  fmrole_inhabited: Inhabited fmrole;
+
+  fmtrans: fmstate → ((fmrole * fmaction) + fmconfig) → fmstate → Prop;
+  fmfairness : trace fmstate ((fmrole * fmaction) + fmconfig) → Prop;
+  live_roles: fmstate → gset fmrole;
+  fm_live_spec: ∀ s ρ α s', fmtrans s (inl (ρ,α)) s' → ρ ∈ live_roles s;
+}.
+
+#[global] Existing Instance fmstate_eqdec.
+#[global] Existing Instance fmstate_inhabited.
+#[global] Existing Instance fmrole_eqdec.
+#[global] Existing Instance fmrole_countable.
+#[global] Existing Instance fmrole_inhabited.
+
+Definition fmlabel (FM :FairModel) : Type :=
+  (fmrole FM * fmaction FM) + fmconfig FM.
+
+Definition fair_model_to_model (FM : FairModel) : Model :=
+  {|
+    mstate := fmstate FM;
+    mlabel := fmlabel FM;
+    mtrans := fmtrans FM;
+  |}.
+
+(* Basically, soundness of the logic and the lemmas above tell us that we have a program
+   trace and a model trace which are related by traces_match labels_math!
+
+   We now prove that this relation transports the properties we care about; the first
+   place of which is fairness.
+ *)
+
+(* Definition of fairness for both kinds of traces *)
+
+Definition mtrace (M:FairModel) :=
+  trace (M.(fmstate)) (fmlabel M).
+
+Section model_traces.
+  Context `{M: FairModel}.
+
+  Definition role_enabled_model ρ (s: M.(fmstate)) := ρ ∈ M.(live_roles) s.
+
+  Definition live_mdl_role (ρ : fmlabel M) (δ : fmstate M) : Prop :=
+    match ρ with
+    | inl (ρ,_) => role_enabled_model ρ δ
+    (* | inr ζ => config_enabled ζ c.2 *)
+    | inr _ => False
+   end.
+
+  Definition fair_scheduling_mtr ρ : mtrace M → Prop :=
+    trace_implies (λ δ _, live_mdl_role ρ δ)
+                  (λ δ ℓ, ¬ live_mdl_role ρ δ ∨ ℓ = Some ρ).
+
+  Lemma fair_scheduling_mtr_after ℓ tr tr' k:
+    after k tr = Some tr' →
+    fair_scheduling_mtr ℓ tr → fair_scheduling_mtr ℓ tr'.
+  Proof. apply trace_implies_after. Qed.
+
+  Lemma fair_scheduling_mtr_cons ℓ δ ℓ' r:
+    fair_scheduling_mtr ℓ (δ -[ℓ']-> r) → fair_scheduling_mtr ℓ r.
+  Proof. apply trace_implies_cons. Qed.
+
+  Lemma fair_scheduling_mtr_cons_forall δ ℓ' r:
+    (∀ ℓ, fair_scheduling_mtr ℓ (δ -[ℓ']-> r)) → (∀ ℓ, fair_scheduling_mtr ℓ r).
+  Proof. intros Hℓ ℓ. eapply trace_implies_cons. apply Hℓ. Qed.
+
+  Definition fair_scheduling mtr := ∀ ρ, fair_scheduling_mtr ρ mtr.
+  Definition mtrace_fair mtr := fair_scheduling mtr ∧ M.(fmfairness) mtr.
+
+  Inductive mtrace_valid_ind (mtrace_valid_coind: mtrace M → Prop) :
+    mtrace M → Prop :=
+  | mtrace_valid_singleton δ: mtrace_valid_ind _ ⟨δ⟩
+  | mtrace_valid_cons δ ℓ tr:
+      fmtrans _ δ ℓ (trfirst tr) →
+      mtrace_valid_coind tr →
+      mtrace_valid_ind _ (δ -[ℓ]-> tr).
+  Definition mtrace_valid := paco1 mtrace_valid_ind bot1.
+
+  Lemma mtrace_valid_mono :
+    monotone1 mtrace_valid_ind.
+  Proof.
+    unfold monotone1. intros x0 r r' IN LE.
+    induction IN; try (econstructor; eauto; done).
+  Qed.
+  Hint Resolve mtrace_valid_mono : paco.
+
+End model_traces.
+
+Global Hint Resolve mtrace_valid_mono : paco.
+
+Definition extrace Λ := trace (cfg Λ) (ex_label Λ).
+
+Section exec_trace.
+  Context {Λ : language}.
+  Context `{EqDecision (locale Λ)}.
+
+  Definition locale_enabled (ζ : locale Λ) (c: cfg Λ) :=
+    ∃ e, from_locale c.1 ζ = Some e ∧ to_val e = None.
+
+  Definition live_ex_label (ζ : ex_label Λ) (c : cfg Λ) : Prop :=
+    match ζ with
+    | inl (ζ,_) => locale_enabled ζ c
+    (* | inr ζ => config_enabled ζ c.2 *)
+    | inr _ => False
+   end.
+
+  Definition fair_scheduling_ex ζ : extrace Λ → Prop :=
+    trace_implies (λ c _, live_ex_label ζ c)
+                  (λ c otid, ¬ live_ex_label ζ c ∨ otid = Some ζ).
+
+  Lemma fair_scheduling_ex_after ζ tr tr' k:
+    after k tr = Some tr' →
+    fair_scheduling_ex ζ tr → fair_scheduling_ex ζ tr'.
+  Proof. destruct ζ; apply trace_implies_after. Qed.
+
+  Lemma fair_scheduling_ex_cons ζ c ζ' r:
+    fair_scheduling_ex ζ (c -[ζ']-> r) → fair_scheduling_ex ζ r.
+  Proof. destruct ζ; apply trace_implies_cons. Qed.
+
+  CoInductive extrace_valid: extrace Λ → Prop :=
+  | extrace_valid_singleton c: extrace_valid ⟨c⟩
+  | extrace_valid_cons c oζ tr:
+      locale_step c oζ (trfirst tr) →
+      extrace_valid tr →
+      extrace_valid (c -[oζ]-> tr).
+
+  Lemma to_trace_preserves_validity ex iex:
+    extrace_valid (to_trace (trace_last ex) iex) → valid_exec ex →
+    valid_inf_exec ex iex.
+  Proof.
+    revert ex iex. cofix CH. intros ex iex Hexval Hval.
+    rewrite (trace_unfold_fold (to_trace _ _)) in Hexval.
+    destruct iex as [|[??] iex]; first by econstructor. cbn in Hexval.
+    inversion Hexval. simplify_eq.
+    econstructor; try done.
+    - by destruct iex as [|[??]?].
+    - apply CH; eauto. econstructor; try done. by destruct iex as [|[??]?].
+  Qed.
+
+  Lemma from_trace_preserves_validity (extr: extrace Λ) ex:
+    extrace_valid extr →
+    valid_exec ex →
+    trace_last ex = trfirst extr →
+    valid_inf_exec ex (from_trace extr).
+  Proof.
+    revert ex extr. cofix CH. intros ex extr Hexval Hval Heq.
+    rewrite (inflist_unfold_fold (from_trace extr)). destruct extr as [c|c tid tr]; cbn;
+     first by econstructor.
+    inversion Hexval; simplify_eq; econstructor; eauto. apply CH; eauto.
+      by econstructor.
+  Qed.
+
+  Lemma from_trace_preserves_validity_singleton (extr: extrace Λ):
+    extrace_valid extr →
+    valid_inf_exec (trace_singleton (trfirst extr)) (from_trace extr).
+  Proof.
+    intros ?. eapply from_trace_preserves_validity; eauto. econstructor.
+  Qed.
+
+End exec_trace.
