fairneris/ltl_lite.v
@@ -1,0 +1,651 @@
+From Paco Require Import paconotation.
+From trillium.fairness Require Export inftraces.
+
+Declare Scope trace_scope.
+Delimit Scope trace_scope with trace.
+Bind Scope trace_scope with trace.
+
+Definition ltl_pred S L := trace S L → Prop.
+
+Section ltl_constructors.
+  Context {S L : Type}.
+
+  Notation ltl_pred := (ltl_pred S L).
+
+  (* Primitive operators *)
+  Definition trace_now P : ltl_pred := λ tr, pred_at tr 0 P.
+  Definition trace_not P : ltl_pred := λ tr, ¬ P tr.
+  Definition trace_or P Q : ltl_pred := λ tr, P tr ∨ Q tr.
+  Definition trace_next P : ltl_pred :=
+    λ tr, ∃ tr', after 1 tr = Some tr' ∧ P tr'.
+  Inductive trace_until P Q : ltl_pred :=
+  | trace_until_here tr : Q tr -> trace_until P Q tr
+  | trace_until_next s l tr : P (s -[l]-> tr) → trace_until P Q tr → trace_until P Q (s -[l]-> tr).
+
+  (* Derived operators *)
+  Definition trace_and P Q := (trace_not (trace_or (trace_not P) (trace_not Q))).
+  Definition trace_implies P Q := (trace_or (trace_not P) Q).
+  Definition trace_biimplies P Q :=
+    (trace_and (trace_implies P Q) (trace_implies Q P)).
+  Definition trace_true := (trace_now (λ _ _, True)).
+  Definition trace_false := (trace_now (λ _ _,False)).
+  Definition trace_eventually P := (trace_until trace_true P).
+  Definition trace_always P := (trace_not $ trace_eventually (trace_not P)).
+  Definition trace_weak_until (P Q : trace S L → Prop) : ltl_pred :=
+    trace_or (trace_until P Q) (trace_always P).
+
+  (* Custom constructors *)
+  Definition trace_always_eventually_implies
+             (P Q : trace S L → Prop) : ltl_pred :=
+    trace_always (trace_implies P (trace_eventually Q)).
+
+  Definition trace_always_eventually_implies_now
+             (P Q : S → option L → Prop) : ltl_pred :=
+    trace_always_eventually_implies (trace_now P) (trace_now Q).
+
+  Lemma trace_eventually_ind (P P0 : trace S L → Prop) :
+    (∀ tr : trace S L, P tr → P0 tr) →
+    (∀ (s : S) (l : L) (tr : trace S L),
+         trace_eventually P tr → P0 tr → P0 (s -[ l ]-> tr)) →
+    ∀ t : trace S L, trace_eventually P t → P0 t.
+  Proof.
+    intros ? IH ??.
+    eapply (trace_until_ind trace_true); [done|by intros; apply IH|done].
+  Qed.
+
+  Definition trace_suffix_of (tr1 tr2 : trace S L) : Prop :=
+    ∃ n, after n tr2 = Some tr1.
+
+End ltl_constructors.
+
+Arguments trace_eventually_ind : clear implicits.
+
+Notation "○ P" := (trace_next P) (at level 20, right associativity) : trace_scope.
+Notation "□ P" := (trace_always P) (at level 20, right associativity) : trace_scope.
+Notation "◊ P" := (trace_eventually P) (at level 20, right associativity) : trace_scope.
+Notation "↓ P" := (trace_now P) (at level 20, right associativity) : trace_scope.
+Notation "P → Q" := (trace_implies P Q)
+                      (at level 99, Q at level 200,
+                         format "'[' P  →  '/' '[' Q ']' ']'") : trace_scope.
+
+(* TODO: Replace existing library lemma with this *)
+Lemma not_exists_forall_not_alt {A} (P : A → Prop) x : ¬ (∃ x, P x) → ¬ P x.
+Proof. intros Hnex HP; apply Hnex; eauto. Qed.
+
+Section ltl_lemmas.
+  Context {S L : Type}.
+
+  (* TODO: Move this *)
+  Lemma after_is_Some_le (tr : trace S L) n m :
+    m ≤ n → is_Some $ after n tr → is_Some $ after m tr.
+  Proof.
+    revert tr m.
+    induction n; intros tr m Hle.
+    { intros. assert (m = 0) as -> by lia. done. }
+    intros.
+    destruct m; [done|].
+    simpl in *.
+    destruct tr; [done|].
+    apply IHn. lia. done.
+  Qed.
+
+  Lemma after_is_Some_lt (tr : trace S L) n m :
+    m < n → is_Some $ after n tr → is_Some $ after m tr.
+  Proof.
+    revert tr m.
+    induction n; intros tr m Hle.
+    { intros. assert (m = 0) as -> by lia. done. }
+    intros.
+    destruct m; [done|].
+    simpl in *.
+    destruct tr; [done|].
+    apply IHn. lia. done.
+  Qed.
+
+  Lemma after_levis n m (tr1 tr2 tr3: trace S L):
+    n ≤ m →
+    after n tr1 = Some tr2 →
+    after m tr1 = Some tr3 →
+    after (m - n) tr2 = Some tr3.
+  Proof.
+    intros Hle Haftern Hafterm.
+    pose proof (Nat.le_exists_sub n m Hle) as [p [-> Hle']].
+    rewrite Nat.add_comm Nat.sub_add'.
+    by rewrite after_sum Haftern in Hafterm.
+  Qed.
+
+  (** trace_suffix_of lemmas  *)
+
+  Lemma trace_suffix_of_refl (tr : trace S L) :
+    trace_suffix_of tr tr.
+  Proof. by exists 0. Qed.
+
+  Lemma trace_suffix_of_cons_l s l (tr tr' : trace S L) :
+    trace_suffix_of (s -[l]-> tr) tr' → trace_suffix_of tr tr'.
+  Proof.
+    intros [n Hafter]. exists (Datatypes.S n).
+    replace (Datatypes.S n) with (n + 1) by lia.
+    rewrite after_sum'. rewrite Hafter. done.
+  Qed.
+
+  Lemma trace_suffix_of_cons_r s l (tr tr' : trace S L) :
+    trace_suffix_of tr tr' → trace_suffix_of tr (s -[l]-> tr').
+  Proof. intros [n Hafter]. by exists (Datatypes.S n). Qed.
+
+  Lemma trace_suffix_of_trans (tr tr' tr'' : trace S L) :
+    trace_suffix_of tr'' tr' → trace_suffix_of tr' tr → trace_suffix_of tr'' tr.
+  Proof.
+    intros [n Hsuffix1] [m Hsuffix2].
+    exists (n+m). rewrite after_sum. rewrite Hsuffix2.
+    rewrite Hsuffix1. done.
+  Qed.
+
+  (** trace_true lemmas *)
+  
+  Lemma trace_trueI (tr : trace S L) : trace_true tr.
+  Proof. destruct tr; done. Qed.
+
+  (** trace_not lemmas *)
+
+  Lemma trace_notI (P : trace S L → Prop) tr :
+    trace_not P tr ↔ ¬ P tr.
+  Proof. done. Qed.
+
+  Lemma trace_not_idemp (P : trace S L → Prop) (tr : trace S L) :
+    trace_not (trace_not P) tr ↔ P tr.
+  Proof. rewrite /trace_not. split; [apply NNP_P|apply P_NNP]. Qed.
+
+  Lemma trace_not_mono (P Q : trace S L → Prop) tr :
+    (Q tr → P tr) → trace_not P tr → trace_not Q tr.
+  Proof. intros HQP HP HQ. apply HP. by apply HQP. Qed.
+  
+  (** trace_next lemmas *)
+
+  Lemma trace_next_intro (P : trace S L → Prop) s l (tr : trace S L) :
+    P tr → (○ P) (s -[l]-> tr).
+  Proof. intros ?. exists tr. simpl in *. by simplify_eq. Qed.
+
+  Lemma trace_next_elim (P : trace S L → Prop) s l tr :
+    (○ P) (s -[l]-> tr) → P tr.
+  Proof. inversion 1. naive_solver. Qed.
+
+  Lemma trace_next_elim_inv (P : trace S L → Prop) tr :
+    (○ P) tr → ∃ s l tr', tr = s -[l]-> tr' ∧ P tr'.
+  Proof. inversion 1. destruct tr; naive_solver. Qed.
+
+  (** trace_implies lemmas *)
+
+  Lemma trace_impliesI (P Q : trace S L → Prop) tr :
+    trace_implies P Q tr ↔ (P tr → Q tr).
+  Proof.
+    split; [by intros [|]|].
+    intros HPQ.
+    assert (P tr ∨ ¬ P tr) as [HP|HP] by apply ExcludedMiddle.
+    + by right; apply HPQ.
+    + by left.
+  Qed.
+
+  Lemma trace_implies_refl (P : trace S L → Prop) tr :
+    trace_implies P P tr.
+  Proof. by apply trace_impliesI. Qed.
+
+  (** trace_or lemmas *)
+
+  Lemma trace_orI (P Q : trace S L → Prop) (tr : trace S L) :
+    trace_or P Q tr ↔ P tr ∨ Q tr.
+  Proof. done. Qed.
+
+  Lemma trace_or_l (P Q : trace S L → Prop) (tr : trace S L) :
+    P tr → trace_or P Q tr.
+  Proof. intros HP. by left. Qed.
+
+  Lemma trace_or_r (P Q : trace S L → Prop) (tr : trace S L) :
+    Q tr → trace_or P Q tr.
+  Proof. intros HP. by right. Qed.
+
+  (** trace_and lemmas *)
+
+  Lemma trace_andI (P Q : trace S L → Prop) (tr : trace S L) :
+    trace_and P Q tr ↔ P tr ∧ Q tr.
+  Proof.
+    split.
+    - intros HPQ.
+      assert (P tr ∨ ¬ P tr) as [HP|HP] by apply ExcludedMiddle; last first.
+      { eapply trace_not_mono in HPQ; [|by apply trace_or_l]. done. }
+      assert (Q tr ∨ ¬ Q tr) as [HQ|HQ] by apply ExcludedMiddle; last first.
+      { eapply trace_not_mono in HPQ; [|by apply trace_or_r]. done. }
+      done.
+    - intros [HP HQ] [HP'|HQ']; done.
+  Qed.
+
+  (** trace_now lemmas *)
+
+  Definition trfirst_label (tr: trace S L) : option L :=
+    match tr with
+    | ⟨_⟩ => None
+    | _ -[ℓ]-> _ => Some ℓ
+    end.
+
+  Lemma trace_now_mono_strong (P Q : S → option L → Prop) tr :
+    (∀ s l, trfirst tr = s → trfirst_label tr = l → P s l → Q s l) →
+    (↓P) tr → (↓Q) tr.
+  Proof.
+    destruct tr as [s|s l tr].
+    - rewrite /trace_now /pred_at /=. intros HPQ Htr. by apply HPQ.
+    - rewrite /trace_now /pred_at /=. intros HPQ Htr. by apply HPQ.
+  Qed.
+
+  Lemma trace_now_mono (P Q : S → option L → Prop) tr :
+    (∀ s l, P s l → Q s l) → (↓P) tr → (↓Q) tr.
+  Proof. intros. eapply trace_now_mono_strong; [|done]. by eauto. Qed.
+
+  Lemma trace_now_not P (tr : trace S L) :
+    (↓ (λ s l, ¬ P s l)) tr ↔ trace_not (↓ P) tr.
+  Proof. by destruct tr. Qed.
+
+  Lemma trace_now_exists {A} (P : A → S → option L → Prop) (tr : trace S L) :
+    (↓ (λ s l, ∃ (x:A), P x s l)) tr → ∃ (x:A), (↓ P x) tr.
+  Proof. rewrite /trace_now /pred_at. intros H. by destruct tr. Qed.
+
+  Lemma trace_now_or (P Q : S → option L → Prop) tr :
+    (↓ (P \2/ Q)) tr → (↓ P) tr ∨ (↓ Q) tr.
+  Proof. rewrite /trace_now /pred_at. by destruct tr=>/=. Qed.
+
+  Lemma trace_now_and P Q (tr : trace S L) :
+    (↓ (P /2\ Q)) tr ↔ trace_and (↓P) (↓Q) tr .
+  Proof. rewrite trace_andI. destruct tr; done. Qed.
+
+  (* TODO: Maybe remove *)
+  Lemma trace_now_split P Q (tr : trace S L) :
+    (↓ P) tr → (↓ Q) tr → (↓ (P /2\ Q)) tr.
+  Proof. intros. apply trace_now_and. rewrite trace_andI. done. Qed.
+
+  (** trace_eventually lemmas *)
+
+  Lemma trace_eventually_intro P (tr : trace S L) :
+    P tr → (◊ P) tr.
+  Proof. by constructor 1. Qed.
+
+  Lemma trace_eventually_cons (P : trace S L → Prop) s l (tr : trace S L) :
+    (◊ P) tr → (◊ P) (s -[l]-> tr).
+  Proof. intros. by constructor 2. Qed.
+
+  Lemma trace_eventually_idemp (P : trace S L → Prop) (tr : trace S L) :
+    (◊◊P) tr → (◊P) tr.
+  Proof.
+    intros Htr. induction Htr using trace_eventually_ind; [done|].
+    apply trace_eventually_cons. done.
+  Qed.
+
+  Lemma trace_eventuallyI_alt (P : trace S L → Prop) tr :
+    (◊ P) tr ↔ (∃ tr', trace_suffix_of tr' tr ∧ (◊ P) tr').
+  Proof.
+    split.
+    - intros Heventually.
+      induction Heventually using trace_eventually_ind.
+      { exists tr. split; [apply trace_suffix_of_refl|].
+        by apply trace_eventually_intro. }
+      destruct IHHeventually as [tr' [Hsuffix HP]].
+      exists tr'.
+      split; [|done].
+      by apply trace_suffix_of_cons_r.
+    - intros [tr' [Hsuffix Htr']].
+      induction Htr' using trace_eventually_ind.
+      { destruct Hsuffix as [n Hafter].
+        revert tr tr0 Hafter H.
+        induction n; intros tr tr0 Hafter HP.
+        { simpl in *. simplify_eq. by apply trace_eventually_intro. }
+        destruct tr; [done|].
+        constructor 2; [done|].
+        by eapply IHn. }
+      apply IHHtr'.
+      by eapply trace_suffix_of_cons_l.
+  Qed.
+
+  Lemma trace_eventuallyI (P : trace S L → Prop) tr :
+    (◊ P) tr ↔ (∃ tr', trace_suffix_of tr' tr ∧ P tr').
+  Proof.
+    split.
+    - intros Heventually.
+      induction Heventually using trace_eventually_ind.
+      { exists tr. split; [apply trace_suffix_of_refl|]. done. }
+      destruct IHHeventually as [tr' [Hsuffix HP]].
+      exists tr'.
+      split; [|done].
+      by apply trace_suffix_of_cons_r.
+    - intros [tr' [Hsuffix Htr']].
+      apply trace_eventuallyI_alt. exists tr'. split=>//.
+      by apply trace_eventually_intro.
+  Qed.
+
+  Lemma trace_eventually_until (P : trace S L → Prop) (tr : trace S L) :
+    (◊P) tr → trace_until (trace_not P) (P) tr.
+  Proof.
+    assert (∀ tr, P tr ∨ ¬ P tr) as Hdec by by intros; apply ExcludedMiddle.
+    induction 1 using trace_eventually_ind; [by constructor|].
+    specialize (Hdec (s -[l]-> tr)) as [H1|H2].
+    - by apply trace_until_here.
+    - by apply trace_until_next.
+  Qed.
+
+  Lemma trace_eventually_mono_strong (P Q : trace S L → Prop) tr :
+    (∀ tr', trace_suffix_of tr' tr → P tr' → Q tr') → (◊P) tr → (◊Q) tr.
+  Proof.
+    intros HPQ.
+    induction 1 using trace_eventually_ind.
+    { apply HPQ, trace_eventually_intro in H. done. apply trace_suffix_of_refl. }
+    constructor 2; [done|].
+    apply IHtrace_eventually.
+    intros tr' Hsuffix HP.
+    apply HPQ; [|done].
+    destruct Hsuffix as [n Heq].
+    exists (Datatypes.S n). done.
+  Qed.
+
+  Lemma trace_eventually_mono (P Q : trace S L → Prop) tr :
+    (∀ tr, P tr → Q tr) → (◊P) tr → (◊Q) tr.
+  Proof.
+    intros. eapply trace_eventually_mono_strong; [|done]. intros. by apply H.
+  Qed.
+
+  Lemma trace_eventually_next (P : trace S L → Prop) (tr : trace S L) :
+    (◊ ○ P) tr → (◊ P) tr.
+  Proof.
+    intros Hnext.
+    induction Hnext using trace_eventually_ind.
+    { destruct tr; [inversion H; naive_solver|].
+      constructor 2; [done|]. constructor. by eapply trace_next_elim. }
+    constructor 2; [done|]. apply IHHnext.
+  Qed.
+
+  Lemma trace_eventually_suffix_of (P : trace S L → Prop) tr1 tr2 :
+    trace_suffix_of tr1 tr2 → (◊P) tr1 → (◊P) tr2.
+  Proof. intros Hsuffix HP. apply trace_eventuallyI_alt. by exists tr1. Qed.
+
+  Lemma trace_eventually_or (P Q : trace S L → Prop) tr :
+    (◊ (P \1/ Q)) tr → (◊ P) tr ∨ (◊ Q) tr.
+  Proof.
+    intros Hdisj.
+    induction Hdisj using trace_eventually_ind.
+    { inversion H; [left; by constructor|right; by constructor]. }
+    inversion IHHdisj.
+    - left. by constructor 2.
+    - right. by constructor 2.
+  Qed.
+
+  (** trace_always lemmas *)
+
+  Lemma trace_always_cons (P : trace S L → Prop) s l (tr : trace S L) :
+    (□ P) (s -[l]-> tr) → (□ P) tr.
+  Proof.
+    intros Htr Htr'. apply Htr. clear Htr. by apply trace_eventually_cons.
+  Qed.
+
+  Lemma trace_always_idemp P (tr : trace S L) :
+    (□ P) tr → (□ □ P) tr.
+  Proof.
+    intros Htr Htr'. induction Htr'; [by apply H|].
+    apply IHHtr'. by apply trace_always_cons in Htr.
+  Qed.
+
+  Lemma trace_always_elim (P : trace S L → Prop) (tr : trace S L) :
+    (□P) tr → P tr.
+  Proof.
+    intros Htr.
+    assert (P tr ∨ ¬ P tr) as [|HP] by apply ExcludedMiddle; [done|].
+    rewrite /trace_always in Htr.
+    assert (trace_not (trace_not P) tr).
+    { intros Htr'. apply Htr. apply trace_eventually_intro. done. }
+    done.
+  Qed.
+
+  Lemma trace_always_mono (P Q : trace S L → Prop) tr :
+    (∀ tr, trace_implies P Q tr) → (□P) tr → (□Q) tr.
+  Proof.
+    intros HPQ HP HQ. apply HP. eapply trace_eventually_mono; [|done].
+    clear HP HQ. intros tr' HP HQ. apply HP.
+    specialize (HPQ tr'). rewrite trace_impliesI in HPQ. by apply HPQ.
+  Qed.
+
+  Lemma trace_always_mono_strong (P Q : trace S L → Prop) tr :
+    (∀ tr', trace_suffix_of tr' tr → trace_implies P Q tr') → (□P) tr → (□Q) tr.
+  Proof.
+    intros HPQ HP HQ. apply HP. eapply trace_eventually_mono_strong; [|done].
+    clear HP HQ. intros tr' Htr' HP HQ. apply HP.
+    specialize (HPQ tr'). rewrite trace_impliesI in HPQ. by apply HPQ.
+  Qed.
+
+  Lemma trace_alwaysI_alt (P : trace S L → Prop) tr :
+    (□P) tr ↔ (∀ tr', trace_suffix_of tr' tr → (□ P) tr').
+  Proof.
+    split.
+    - intros Htr tr' Hsuffix Htr'.
+      apply Htr.
+      induction Htr' using trace_eventually_ind.
+      { eapply trace_eventuallyI_alt. exists tr0. split; [done|].
+        by apply trace_eventually_intro. }
+      apply IHHtr'. by eapply trace_suffix_of_cons_l.
+    - intros Htr' Htr.
+      induction Htr using trace_eventually_ind.
+      { specialize (Htr' tr). apply Htr'.
+        { apply trace_suffix_of_refl. }
+        by apply trace_eventually_intro. }
+      apply IHHtr. intros tr' Htsuffix. apply Htr'.
+      by eapply trace_suffix_of_cons_r.
+  Qed.
+
+  Lemma trace_always_suffix_of (P : trace S L → Prop) tr1 tr2 :
+    trace_suffix_of tr2 tr1 → (□P) tr1 → (□P) tr2.
+  Proof. rewrite (trace_alwaysI_alt _ tr1). intros Hsuffix HP. by eapply HP. Qed.
+
+  Lemma trace_alwaysI (P : trace S L → Prop) tr :
+    (□P) tr ↔ (∀ tr', trace_suffix_of tr' tr → P tr').
+  Proof.
+    split.
+    - intros HP tr' Hsuff. rewrite trace_alwaysI_alt in HP.
+      apply trace_always_elim. eauto.
+    - intros H Habs. apply trace_eventuallyI in Habs as (tr'&Hsuff&?).
+      by specialize (H _ Hsuff).
+  Qed.
+
+  Lemma trace_always_forall {A} (P : A → trace S L → Prop) tr :
+    (∀ (x:A), (□ (P x)) tr) ↔ (□ (λ tr', ∀ x, P x tr')) tr.
+  Proof.
+    split.
+    - intros Htr Htr'.
+      induction Htr' using trace_eventually_ind.
+      { apply H. intros x. specialize (Htr x).
+        apply trace_always_elim in Htr. apply Htr. }
+      apply IHHtr'.
+      intros x. specialize (Htr x).
+      by apply trace_always_cons in Htr.
+    - intros Htr x Htr'.
+      induction Htr' using trace_eventually_ind.
+      { apply H. apply trace_always_elim in Htr. apply Htr. }
+      apply IHHtr'. by apply trace_always_cons in Htr.
+  Qed.
+
+  (* TODO: This breaks naming convention *)
+  Lemma trace_always_universal (P : trace S L → Prop) (tr : trace S L) :
+    (∀ tr, P tr) → (□P) tr.
+  Proof.
+    intros ? H. induction H using trace_eventually_ind; [|done].
+    simplify_eq. specialize (H0 tr). done.
+  Qed.
+
+  (* TODO: This is a bit of a weird statement *)
+  Lemma trace_always_implies (P Q : trace S L → Prop) tr :
+    (□(P → Q)) tr → (□P) tr → (□ Q) tr.
+  Proof.
+    intros HPQ HP.
+    eapply trace_always_mono_strong; [|done].
+    intros tr' Hsuffix.
+    apply trace_always_elim.
+    by eapply trace_always_suffix_of.
+  Qed.
+
+  Lemma trace_always_eventually P (tr : trace S L) :
+    (□ P) tr → (◊ P) tr.
+  Proof.
+    intros Halways. eapply trace_eventuallyI_alt. exists tr.
+    split; [apply trace_suffix_of_refl|]. apply trace_eventually_intro.
+    by apply trace_always_elim in Halways.
+  Qed.
+
+  Lemma trace_always_eventually_suffix_of tr1 tr2 (P : trace S L → Prop) :
+    trace_suffix_of tr1 tr2 → (□◊ P) tr1 → (□◊ P) tr2.
+  Proof.
+    intros [n Hn] H1.
+    apply trace_alwaysI.
+    intros tr' [m Hm].
+    apply trace_eventuallyI_alt.
+    destruct (decide (m ≤ n)).
+    - exists tr1. split.
+      + exists (n - m). eapply after_levis =>//.
+      + by apply trace_always_elim in H1.
+    - exists tr'. split=>//.
+      + exists 0. done.
+      + assert (Hsuff: trace_suffix_of tr' tr1).
+        * exists (m - n). assert (n ≤ m) by lia. eapply after_levis =>//.
+        * rewrite trace_alwaysI_alt in H1. specialize (H1 tr' Hsuff).
+          by apply trace_always_elim in H1.
+  Qed.
+
+  Lemma trace_always_eventually_always_implies (P Q : trace S L → Prop) tr :
+    trace_always_eventually_implies P Q tr → (□P) tr → (◊Q) tr.
+  Proof.
+    intros HPQ HP.
+    eapply trace_always_implies in HP; [|done].
+    by apply trace_always_elim.
+  Qed.
+
+  Lemma trace_always_eventually_always_mono (P1 P2 Q1 Q2 : trace S L → Prop) tr :
+    (∀ tr, trace_implies P2 P1 tr) → (∀ tr, trace_implies Q1 Q2 tr) →
+    trace_always_eventually_implies P1 Q1 tr → trace_always_eventually_implies P2 Q2 tr.
+  Proof.
+    setoid_rewrite trace_impliesI.
+    intros HP HQ Htr.
+    eapply trace_always_mono; [|done].
+    intros Htr'.
+    apply trace_impliesI.
+    rewrite !trace_impliesI.
+    intros HPQ HP2.
+    eapply trace_eventually_mono; [apply HQ|by apply HPQ; apply HP].
+  Qed.
+
+  Lemma trace_always_not_not_eventually (P : trace S L → Prop) (tr : trace S L) :
+    (□ (trace_not P)) tr ↔ trace_not (◊ P) tr.
+  Proof.
+    split.
+    - intros Halways Heventually.
+      induction Heventually.
+      { apply Halways. apply trace_eventually_intro. by apply P_NNP. }
+      apply IHHeventually.
+      by apply trace_always_cons in Halways.
+    - intros Heventually Halways.
+      induction Halways using trace_eventually_ind.
+      { apply Heventually. apply trace_eventually_intro.
+        eapply trace_not_mono in Heventually; [|by apply trace_eventually_intro].
+        done. }
+      apply IHHalways.
+      intros Heventually'. apply Heventually. by apply trace_eventually_cons.
+  Qed.
+
+  Lemma trace_eventually_not_not_always (P : trace S L → Prop) (tr : trace S L) :
+    (◊ trace_not P) tr ↔ (trace_not (□ P)) tr.
+  Proof.
+    split.
+    - intros Heventually. apply P_NNP. done.
+    - intros Halways. apply NNP_P in Halways. done.
+  Qed.
+
+  Lemma trace_always_and P Q (tr : trace S L) :
+    (□ trace_and P Q) tr ↔ ((□ P) tr ∧ (□ Q) tr).
+  Proof.
+    split.
+    - intros HPQ.
+      assert ((□ P) tr ∨ ¬ (□ P) tr) as [|HP] by apply ExcludedMiddle; last first.
+      { apply NNP_P in HP. induction HP using trace_eventually_ind.
+        { apply trace_always_elim in HPQ. apply trace_andI in HPQ as [HP HQ].
+          done. }
+        apply trace_always_cons in HPQ. apply IHHP in HPQ.
+        destruct HPQ as [HP' HQ].
+        apply trace_eventually_not_not_always in HP. done. }
+      assert ((□ Q) tr ∨ ¬ (□ Q) tr) as [|HQ] by apply ExcludedMiddle; last first.
+      { apply NNP_P in HQ. induction HQ using trace_eventually_ind.
+        { apply trace_always_elim in HPQ. apply trace_andI in HPQ as [HP HQ].
+          done. }
+        apply trace_always_cons in HPQ.
+        apply trace_always_cons in H.
+        apply IHHQ in HPQ; [|done].
+        destruct HPQ as [HP HQ'].
+        apply trace_eventually_not_not_always in HQ. done. }
+      done.
+    - intros [HP HQ] HPQ. induction HPQ.
+      { apply H. apply trace_andI. apply trace_always_elim in HP, HQ. done. }
+      by apply IHHPQ; eapply trace_always_cons.
+  Qed.
+
+  Lemma trace_weak_until_always P Q (tr : trace S L) :
+    (□P) tr → trace_weak_until P Q tr.
+  Proof. intros HP. by apply trace_or_r. Qed.
+
+  (* TODO: Remove? *)
+  Lemma trace_always_implies_always (P Q : trace S L → Prop) (tr : trace S L) :
+    (∀ tr, (□P) tr → Q tr) → ((□P) tr → (□ Q) tr).
+  Proof.
+    intros HPQ HP%trace_always_idemp. eapply trace_always_mono; [|done].
+    intros ?. apply trace_impliesI, HPQ.
+  Qed.
+
+End ltl_lemmas.
+
+Section ltl_theorems.
+  Context {S L : Type}.
+
+  (* Strong fairness implies our (network) fairness *)
+  Lemma SF_implies_OF (P Q: trace S L → Prop) tr :
+    ((□◊ P) → (□◊ Q))%trace tr → (□ ((□◊ P) → (◊ Q))) tr.
+  Proof.
+    intros Hsf. apply trace_alwaysI. intros tr' Hsuff.
+    apply trace_impliesI. intros Hae.
+    eapply trace_always_eventually_suffix_of in Hae =>//.
+    rewrite trace_impliesI in Hsf. specialize (Hsf Hae).
+    apply trace_always_elim. by eapply trace_always_suffix_of.
+  Qed.
+
+  Lemma OF_implies_SF (P Q: trace S L → Prop) tr :
+    (□ ((□◊ P) → (◊ Q))) tr → ((□◊ P) → (□◊ Q))%trace tr.
+  Proof.
+    intros Hsf. apply trace_impliesI.
+    intros HP. apply trace_always_idemp in HP. revert HP.
+    by apply trace_always_implies.
+  Qed.
+
+  Theorem SF_equiv_OF (P Q: trace S L → Prop) tr :
+    ((□◊ P) → (□◊ Q))%trace tr ≡ (□ ((□◊ P) → (◊ Q))) tr.
+  Proof. split; [apply SF_implies_OF|apply OF_implies_SF]. Qed.
+
+  (* Our (scheduling) Fairness implies Strong Fairness *)
+  Lemma OF_implies_SF' (P Q: trace S L → Prop) tr :
+    (□ (P → (◊ Q)))%trace tr → ((□◊ P) → (□◊ Q))%trace tr.
+  Proof.
+    intros Htr. apply trace_impliesI.
+    apply trace_always_implies.
+    rewrite trace_alwaysI_alt in Htr.
+    rewrite trace_alwaysI.
+    intros tr' Hsuffix.
+    specialize (Htr tr' Hsuffix).
+    apply trace_impliesI.
+    intros HP.
+    rewrite trace_eventuallyI in HP.
+    destruct HP as [tr'' [Hsuffix' HP]].
+    rewrite trace_alwaysI in Htr.
+    specialize (Htr tr'' Hsuffix').
+    rewrite trace_impliesI in Htr.
+    rewrite trace_eventuallyI_alt.
+    exists tr''. split; [done|].
+    apply Htr. done.
+  Qed.
+
+End ltl_theorems.
