fairneris/mu_calculus_lite.v
@@ -1,0 +1,61 @@
+From stdpp Require Import option.
+From trillium.fairness Require Export inftraces.
+
+Definition mu_pred (S L : Type) : Type := trace S L → Prop.
+
+Section mu_defs.
+  Context {S L : Type}.
+
+  Notation mu_pred := (mu_pred S L).
+
+  Definition trtail (tr : trace S L) : option (L * trace S L) :=
+    match tr with
+    | ⟨s⟩ => None
+    | s -[ℓ]-> r => Some (ℓ,r)
+    end.
+
+  Definition mu_now (P : S → Prop) : mu_pred :=
+    λ tr, P $ trfirst tr.
+  Definition mu_box (P : L → Prop) (ϕ : mu_pred) : mu_pred := 
+    λ tr, ∃ l tr', trtail tr = Some (l, tr') ∧ P l ∧ ϕ tr'.
+
+  Definition mu_pred_mono (F : mu_pred → mu_pred) : Prop :=
+    ∀ (ϕ ψ : mu_pred), (∀ tr, ϕ tr → ψ tr) → (∀ tr, F ϕ tr → F ψ tr).
+
+  Definition mu_mu {A} (F : (A → Prop) → (A → Prop)) : (A → Prop) :=
+    λ tr, ∃ (ϕ : (A → Prop)), (∀ tr, ϕ tr → F ϕ tr) ∧ ϕ tr.
+  Definition mu_nu  {A} (F : (A → Prop) → (A → Prop)) : (A → Prop) :=
+    λ tr, ∀ (ϕ : (A → Prop)), (∀ tr, F ϕ tr → ϕ tr) → ϕ tr.
+
+  (* Definition mu_mu (F : mu_pred → mu_pred) : mu_pred := *)
+  (*   λ tr, ∃ (ϕ : mu_pred), (∀ tr, ϕ tr → F ϕ tr) ∧ ϕ tr. *)
+  (* Definition mu_nu (F : mu_pred → mu_pred) : mu_pred := *)
+  (*   λ tr, ∀ (ϕ : mu_pred), (∀ tr, F ϕ tr → ϕ tr) → ϕ tr. *)
+
+  Class MonoPred {A : Type} (F : (A → Prop) → (A → Prop)) := {
+      mono_pred (Φ Ψ : A → Prop) : (∀ x, Φ x → Ψ x) → ∀ x, F Φ x → F Ψ x;
+    }.
+  
+  Lemma least_fixpoint_unfold_2 {A} (F : (A → Prop) → (A → Prop)) `{!MonoPred F} x :
+    F (mu_nu F) x → mu_nu F x.
+  Proof using Type*.
+    rewrite /mu_nu /=. intros HF ϕ Hincl.
+    apply Hincl. eapply mono_pred; [|by apply HF].
+    intros y H'. apply H'. apply Hincl.
+  Qed.
+
+  Lemma least_fixpoint_unfold_1 {A} (F : (A → Prop) → (A → Prop)) `{!MonoPred F} x :
+    mu_nu F x → F (mu_nu F) x.
+  Proof using Type*.
+    intros HF. apply HF.
+    intros y Hy. eapply mono_pred; [|by apply HF].
+    intros z ?. by apply least_fixpoint_unfold_2.
+  Qed.
+
+  Corollary least_fixpoint_unfold {A} (F : (A → Prop) → (A → Prop)) `{!MonoPred F} x :
+    mu_nu F x ↔ F (mu_nu F) x.
+  Proof using Type*.
+    split; [by apply least_fixpoint_unfold_1|by apply least_fixpoint_unfold_2].
+  Qed.
+
+End mu_defs.
