trillium/program_logic/ectxi_language.v
@@ -26,13 +26,14 @@ Below you can find the relevant parts:
 *)
 
 Section ectxi_language_mixin.
-  Context {expr val ectx_item state locale : Type}.
+  Context {expr val ectx_item state locale action config_label : Type}.
   Context (of_val : val → expr).
   Context (to_val : expr → option val).
   Context (fill_item : ectx_item → expr → expr).
-  Context (head_step : expr → state → expr → state → list expr → Prop).
-  Context (config_step : state → state → Prop).
-  Context (locale_of : list expr -> expr -> locale).
+  Context (head_step : expr → state → action → expr → state → list expr → Prop).
+  Context (config_step : state → config_label → state → Prop).
+  Context (locale_of : list expr → expr → locale).
+  (* Context (config_enabled : config_label → state → Prop). *)
 
   Notation locales_equiv t0 t0' :=
     (Forall2 (λ '(t, e) '(t', e'), locale_of t e = locale_of t' e') (prefixes t0) (prefixes t0')).
@@ -40,7 +41,7 @@ Section ectxi_language_mixin.
   Record EctxiLanguageMixin := {
     mixin_to_of_val v : to_val (of_val v) = Some v;
     mixin_of_to_val e v : to_val e = Some v → of_val v = e;
-    mixin_val_stuck e1 σ1 e2 σ2 efs : head_step e1 σ1 e2 σ2 efs → to_val e1 = None;
+    mixin_val_stuck e1 σ1 α e2 σ2 efs : head_step e1 σ1 α e2 σ2 efs → to_val e1 = None;
 
     mixin_fill_item_val Ki e : is_Some (to_val (fill_item Ki e)) → is_Some (to_val e);
     (** [fill_item] is always injective on the expression for a fixed
@@ -56,15 +57,17 @@ Section ectxi_language_mixin.
         [ectx_language], an empty context is impossible here).  In other words,
         if [e] is not a value then wrapping it in a context does not add new
         head redex positions. *)
-    mixin_head_ctx_step_val Ki e σ1 e2 σ2 efs :
-      head_step (fill_item Ki e) σ1 e2 σ2 efs → is_Some (to_val e);
+    mixin_head_ctx_step_val Ki e σ1 α e2 σ2 efs :
+      head_step (fill_item Ki e) σ1 α e2 σ2 efs → is_Some (to_val e);
 
-    mixin_locale_step e1 e2 t1 σ1 σ2 efs: head_step e1 σ1 e2 σ2 efs ->
+    mixin_locale_step e1 e2 t1 σ1 α σ2 efs: head_step e1 σ1 α e2 σ2 efs ->
                                          locale_of t1 e1 = locale_of t1 e2;
     mixin_locale_fill e K t1: locale_of t1 (fill_item K e) = locale_of t1 e;
     mixin_locale_equiv t t' e: locales_equiv t t' -> locale_of t e = locale_of t' e;
     mixin_locale_injective tp0 e0 tp1 tp e:
       (tp, e) ∈ prefixes_from (tp0 ++ [e0]) tp1 -> locale_of tp0 e0 ≠ locale_of tp e;
+    (* mixin_config_enabled σ lbl : *)
+    (*   (∃ σ', config_step σ lbl σ') ↔ config_enabled lbl σ; *)
   }.
 End ectxi_language_mixin.
 
@@ -74,28 +77,32 @@ Structure ectxiLanguage := EctxiLanguage {
   ectx_item : Type;
   state : Type;
   locale : Type;
+  action : Type;
+  config_label : Type;
 
   of_val : val → expr;
   to_val : expr → option val;
   fill_item : ectx_item → expr → expr;
-  head_step : expr → state → expr → state → list expr → Prop;
-  config_step : state → state → Prop;
-  locale_of : list expr -> expr -> locale;
+  head_step : expr → state → action → expr → state → list expr → Prop;
+  config_step : state → config_label → state → Prop;
+  locale_of : list expr → expr → locale;
+  (* config_enabled : config_label → state → Prop; *)
 
   ectxi_language_mixin :
-    EctxiLanguageMixin of_val to_val fill_item head_step locale_of
+    EctxiLanguageMixin of_val to_val fill_item head_step (* config_step *) locale_of (* config_enabled *)
 }.
 
 Bind Scope expr_scope with expr.
 Bind Scope val_scope with val.
 
-Arguments EctxiLanguage {_ _ _ _ _ _ _ _} _ _.
+Arguments EctxiLanguage {_ _ _ _ _ _ _ _ _ _} _ _ _ _.
 Arguments of_val {_} _.
 Arguments to_val {_} _.
 Arguments fill_item {_} _ _.
 Arguments head_step {_} _ _ _ _ _.
-Arguments config_step {_} _ _.
+Arguments config_step {_} _ _ _.
 Arguments locale_of {_} _ _.
+(* Arguments config_enabled {_} _ _. *)
 
 Section ectxi_language.
   Context {Λ : ectxiLanguage}.
@@ -111,8 +118,8 @@ Section ectxi_language.
     to_val e1 = None → to_val e2 = None →
     fill_item Ki1 e1 = fill_item Ki2 e2 → Ki1 = Ki2.
   Proof. apply ectxi_language_mixin. Qed.
-  Lemma head_ctx_step_val Ki e σ1 e2 σ2 efs :
-    head_step (fill_item Ki e) σ1 e2 σ2 efs → is_Some (to_val e).
+  Lemma head_ctx_step_val Ki e σ1 α e2 σ2 efs :
+    head_step (fill_item Ki e) σ1 α e2 σ2 efs → is_Some (to_val e).
   Proof. apply ectxi_language_mixin. Qed.
 
   Definition fill (K : ectx) (e : expr Λ) : expr Λ := foldl (flip fill_item) e K.
@@ -121,7 +128,7 @@ Section ectxi_language.
   Proof. apply foldl_app. Qed.
 
   Definition ectxi_lang_ectx_mixin :
-    EctxLanguageMixin of_val to_val [] (flip (++)) fill head_step locale_of.
+    EctxLanguageMixin of_val to_val [] (flip (++)) fill head_step (* config_step *) locale_of (* config_enabled *).
   Proof.
     assert (fill_val : ∀ K e, is_Some (to_val (fill K e)) → is_Some (to_val e)).
     { intros K. induction K as [|Ki K IH]=> e //=. by intros ?%IH%fill_item_val. }
@@ -148,7 +155,7 @@ Section ectxi_language.
       apply IHK in Hes as [[Kx ->]|[Kx ->]]; [| |done|done].
       + left; eexists; rewrite -assoc; done.
       + right; eexists; rewrite -assoc; done.
-    - intros K K' e1 e1' σ1 e2 σ2 efs Hfill Hred Hstep; revert K' Hfill.
+    - intros K K' e1 e1' α σ1 e2 σ2 efs Hfill Hred Hstep; revert K' Hfill.
       induction K as [|Ki K IH] using rev_ind=> /= K' Hfill; eauto using app_nil_r.
       destruct K' as [|Ki' K' _] using @rev_ind; simplify_eq/=.
       { rewrite fill_app in Hstep. apply head_ctx_step_val in Hstep.
@@ -159,7 +166,7 @@ Section ectxi_language.
         apply fill_not_val. revert Hstep. apply ectxi_language_mixin. }
       simplify_eq. destruct (IH K') as [K'' ->]; auto.
       exists K''. by rewrite assoc.
-    - intros K e1 σ1 e2 σ2 efs.
+    - intros K e1 σ1 α e2 σ2 efs.
       destruct K as [|Ki K _] using rev_ind; simpl; first by auto.
       rewrite fill_app /=.
       intros ?%head_ctx_step_val; eauto using fill_val.
@@ -168,9 +175,10 @@ Section ectxi_language.
       intros e t1. rewrite IH. apply ectxi_language_mixin.
     - apply ectxi_language_mixin.
     - apply ectxi_language_mixin.
+    (* - apply ectxi_language_mixin. *)
   Qed.
 
-  Canonical Structure ectxi_lang_ectx := EctxLanguage head_step config_step locale_of ectxi_lang_ectx_mixin.
+  Canonical Structure ectxi_lang_ectx := EctxLanguage head_step config_step locale_of (* config_enabled *) ectxi_lang_ectx_mixin.
   Canonical Structure ectxi_lang := LanguageOfEctx ectxi_lang_ectx.
 
   Lemma fill_not_val K e : to_val e = None → to_val (fill K e) = None.
@@ -192,7 +200,7 @@ Coercion ectxi_lang_ectx : ectxiLanguage >-> ectxLanguage.
 Coercion ectxi_lang : ectxiLanguage >-> language.
 
 Definition EctxLanguageOfEctxi (Λ : ectxiLanguage) : ectxLanguage :=
-  let '@EctxiLanguage E V C St L of_val to_val fill head config locale_of mix := Λ in
-  @EctxLanguage E V (list C) St L of_val to_val _ _ _ _ config locale_of
+  let '@EctxiLanguage E V C St L action config_label of_val to_val fill head config locale_of (* config_enabled *) mix := Λ in
+  @EctxLanguage E V (list C) St L action config_label of_val to_val _ _ _ _ config locale_of (* config_enabled *)
     (@ectxi_lang_ectx_mixin
-       (@EctxiLanguage E V C St L of_val to_val fill head config locale_of mix)).
+       (@EctxiLanguage E V C St L action config_label of_val to_val fill head config locale_of (* config_enabled *) mix)).
