trillium/program_logic/lifting.v
@@ -23,10 +23,10 @@ Lemma wp_lift_step_fupdN s E Φ e1 ζ:
     ⌜locale_of tp1 (ectx_fill K e1) = ζ⌝ -∗
     state_interp extr atr ={E,∅}=∗
     ⌜if s is NotStuck then reducible e1 σ1 else True⌝ ∗
-    ∀ e2 σ2 efs, ⌜prim_step e1 σ1 e2 σ2 efs⌝ ={∅}▷=∗^(S $ trace_length extr) |={∅,E}=>
+    ∀ α e2 σ2 efs, ⌜prim_step e1 σ1 α e2 σ2 efs⌝ ={∅}▷=∗^(S $ trace_length extr) |={∅,E}=>
      ∃ δ2 ℓ,
        state_interp
-         (trace_extend extr (Some ζ) (tp1 ++ ectx_fill K e2 :: tp2 ++ efs, σ2))
+         (trace_extend extr (inl (ζ,α)) (tp1 ++ ectx_fill K e2 :: tp2 ++ efs, σ2))
          (trace_extend atr ℓ δ2) ∗
         WP e2 @ s; ζ; E {{ Φ }} ∗
         [∗ list] i ↦ef ∈ efs, WP ef @ s; locale_of (tp1 ++ ectx_fill K e1 :: tp2 ++ (take i efs)) ef; ⊤
@@ -36,7 +36,7 @@ Proof.
   rewrite wp_unfold /wp_pre=>->.
   iIntros "H" (exre atr K tp1 tp2 σ1 Hexvald Hlocale Hexe) "Hsi".
   iMod ("H" with "[//] [//] [//] Hsi") as "[$ H]".
-  iIntros "!#" (e2 σ2 efs Hstep).
+  iIntros "!#" (α e2 σ2 efs Hstep).
   iMod ("H" with "[//]") as "H".
   iModIntro; iNext.
   iApply "H".
@@ -50,17 +50,17 @@ Lemma wp_lift_step_fupd s E Φ e1 ζ:
     ⌜locale_of tp1 (ectx_fill K e1) = ζ⌝ -∗
     state_interp extr atr ={E,∅}=∗
     ⌜if s is NotStuck then reducible e1 σ1 else True⌝ ∗
-    ∀ e2 σ2 efs, ⌜prim_step e1 σ1 e2 σ2 efs⌝ ={∅}=∗ ▷ |={∅,E}=>
+    ∀ α e2 σ2 efs, ⌜prim_step e1 σ1 α e2 σ2 efs⌝ ={∅}=∗ ▷ |={∅,E}=>
      ∃ δ2 ℓ,
        state_interp
-         (trace_extend extr (Some ζ) (tp1 ++ ectx_fill K e2 :: tp2 ++ efs, σ2))
+         (trace_extend extr (inl (ζ,α)) (tp1 ++ ectx_fill K e2 :: tp2 ++ efs, σ2))
          (trace_extend atr ℓ δ2) ∗
         WP e2 @ s; ζ; E {{ Φ }} ∗
         [∗ list] i ↦ef ∈ efs, WP ef @ s; locale_of (tp1 ++ ectx_fill K e1 :: tp2 ++ (take i efs)) ef; ⊤
            {{ fork_post (locale_of (tp1 ++ ectx_fill K e1 :: tp2 ++ (take i efs)) ef) }})
   ⊢ WP e1 @ s; ζ; E {{ Φ }}.
 Proof.
-    intros ?. rewrite -wp_lift_step_fupdN; [|done]. simpl. do 26 f_equiv.
+    intros ?. rewrite -wp_lift_step_fupdN; [|done]. simpl. do 28 f_equiv.
     rewrite -step_fupdN_intro; [|done]. rewrite -bi.laterN_intro. auto.
 Qed.
 
@@ -76,7 +76,7 @@ Proof.
   iIntros "H" (ex atr K tp1 tp2 σ Hexvalid Hlocale  Hex) "Hsi".
   iMod ("H" with "[//] [//] Hsi") as %[? Hirr].
   iModIntro. iSplit; first done.
-  iIntros (e2 σ2 efs ?). by case: (Hirr e2 σ2 efs).
+  iIntros (α e2 σ2 efs ?). by case: (Hirr α e2 σ2 efs).
  Qed.
 
 (** Derived lifting lemmas. *)
@@ -88,10 +88,10 @@ Lemma wp_lift_step s E Φ e1 ζ:
     ⌜locale_of tp1 (ectx_fill K e1) = ζ⌝ -∗
     state_interp extr atr ={E,∅}=∗
     ⌜if s is NotStuck then reducible e1 σ1 else True⌝ ∗
-    ▷ ∀ e2 σ2 efs, ⌜prim_step e1 σ1 e2 σ2 efs⌝ ={∅,E}=∗
+    ▷ ∀ α e2 σ2 efs, ⌜prim_step e1 σ1 α e2 σ2 efs⌝ ={∅,E}=∗
       ∃ δ2 ℓ, 
         state_interp
-          (trace_extend extr (Some ζ) (tp1 ++ ectx_fill K e2 :: tp2 ++ efs, σ2))
+          (trace_extend extr (inl (ζ,α)) (tp1 ++ ectx_fill K e2 :: tp2 ++ efs, σ2))
           (trace_extend atr ℓ δ2) ∗
       WP e2 @ s; ζ; E {{ Φ }} ∗
       [∗ list] i ↦ef ∈ efs, WP ef @ s; locale_of (tp1 ++ ectx_fill K e1 :: tp2 ++ (take i efs)) ef; ⊤
@@ -106,8 +106,8 @@ Qed.
 Lemma wp_lift_pure_step_no_fork
       `{!AllowsPureStep M Σ} `{!Inhabited (state Λ)} s E E' Φ e1 ζ:
   (∀ σ1, if s is NotStuck then reducible e1 σ1 else to_val e1 = None) →
-  (∀ σ1 e2 σ2 efs, prim_step e1 σ1 e2 σ2 efs → σ2 = σ1 ∧ efs = []) →
-  (|={E}[E']▷=> ∀ e2 efs σ, ⌜prim_step e1 σ e2 σ efs⌝ → WP e2 @ s; ζ; E {{ Φ }})
+  (∀ σ1 α e2 σ2 efs, prim_step e1 σ1 α e2 σ2 efs → σ2 = σ1 ∧ efs = []) →
+  (|={E}[E']▷=> ∀ α e2 efs σ, ⌜prim_step e1 σ α e2 σ efs⌝ → WP e2 @ s; ζ; E {{ Φ }})
   ⊢ WP e1 @ s; ζ; E {{ Φ }}.
 Proof.
   iIntros (Hsafe Hstep) "H". iApply wp_lift_step.
@@ -116,8 +116,8 @@ Proof.
   iMod fupd_mask_subseteq as "Hclose"; last iModIntro; first by set_solver.
   iSplit.
   { iPureIntro. destruct s; done. }
-  iNext. iIntros (e2 σ2 efs ?).
-  destruct (Hstep σ1 e2 σ2 efs) as (<- & ->); auto.
+  iNext. iIntros (α e2 σ2 efs ?).
+  destruct (Hstep σ1 α e2 σ2 efs) as (<- & ->); auto.
   iMod "Hclose" as "_". iMod "H".
   iMod (allows_pure_step with "Hsi") as "Hsi"; [done|done|done| |].
   { econstructor 1; [done| |by apply fill_step]; by rewrite app_nil_r. }
@@ -149,10 +149,10 @@ Lemma wp_lift_atomic_step_fupd {s E1 E2 Φ} e1 ζ:
     ⌜locale_of tp1 e1 = ζ⌝ →
     state_interp extr atr ={E1}=∗
     ⌜if s is NotStuck then reducible e1 σ1 else True⌝ ∗
-    ∀ e2 σ2 efs, ⌜prim_step e1 σ1 e2 σ2 efs⌝ ={E1}[E2]▷=∗
+    ∀ α e2 σ2 efs, ⌜prim_step e1 σ1 α e2 σ2 efs⌝ ={E1}[E2]▷=∗
       ∃ δ2 ℓ, 
         state_interp
-          (trace_extend extr (Some ζ) (tp1 ++ ectx_fill K e2 :: tp2 ++ efs, σ2))
+          (trace_extend extr (inl (ζ,α)) (tp1 ++ ectx_fill K e2 :: tp2 ++ efs, σ2))
           (trace_extend atr ℓ δ2) ∗
       from_option Φ False (to_val e2) ∗
       [∗ list] i ↦ef ∈ efs, WP ef @ s; locale_of (tp1 ++ ectx_fill K e1 :: tp2 ++ (take i efs)) ef; ⊤
@@ -165,8 +165,8 @@ Proof.
   iMod ("H" with "[//] [//] [] Hsi") as "[$ H]".
   { iPureIntro. by erewrite <-locale_fill. }
   iMod (fupd_mask_subseteq ∅) as "Hclose"; first set_solver.
-  iIntros "!>" (e2 σ2 efs ?). iMod "Hclose" as "_".
-  iMod ("H" $! e2 σ2 efs with "[#]") as "H"; [done|].
+  iIntros "!>" (α e2 σ2 efs ?). iMod "Hclose" as "_".
+  iMod ("H" $! α e2 σ2 efs with "[#]") as "H"; [done|].
   iMod (fupd_mask_subseteq ∅) as "Hclose"; [set_solver|]. iIntros "!> !>".
   iMod "Hclose" as "_". iMod "H" as (st' ℓ) "(? & HQ & $)".
   destruct (to_val e2) eqn:?; last by iExFalso.
@@ -183,10 +183,10 @@ Lemma wp_lift_atomic_step {s E Φ} e1 ζ:
     ⌜locale_of tp1 e1 = ζ⌝ →
     state_interp extr atr ={E}=∗
     ⌜if s is NotStuck then reducible e1 σ1 else True⌝ ∗
-    ▷ ∀ e2 σ2 efs, ⌜prim_step e1 σ1 e2 σ2 efs⌝ ={E}=∗
+    ▷ ∀ α e2 σ2 efs, ⌜prim_step e1 σ1 α e2 σ2 efs⌝ ={E}=∗
       ∃ δ2 ℓ, 
         state_interp
-          (trace_extend extr (Some ζ) (tp1 ++ ectx_fill K e2 :: tp2 ++ efs, σ2))
+          (trace_extend extr (inl (ζ,α)) (tp1 ++ ectx_fill K e2 :: tp2 ++ efs, σ2))
           (trace_extend atr ℓ δ2) ∗
       from_option Φ False (to_val e2) ∗
       [∗ list] i ↦ef ∈ efs, WP ef @ s; locale_of (tp1 ++ ectx_fill K e1 :: tp2 ++ (take i efs)) ef; ⊤
@@ -202,14 +202,14 @@ Qed.
 Lemma wp_lift_pure_det_step_no_fork
       `{!AllowsPureStep M Σ} `{!Inhabited (state Λ)} {s E E' Φ} e1 e2 ζ:
   (∀ σ1, if s is NotStuck then reducible e1 σ1 else to_val e1 = None) →
-  (∀ σ1 e2' σ2 efs', prim_step e1 σ1 e2' σ2 efs' →
+  (∀ σ1 α e2' σ2 efs', prim_step e1 σ1 α e2' σ2 efs' →
     σ2 = σ1 ∧ e2' = e2 ∧ efs' = []) →
   (|={E}[E']▷=> WP e2 @ s; ζ; E {{ Φ }}) ⊢ WP e1 @ s; ζ; E {{ Φ }}.
 Proof.
   iIntros (? Hpuredet) "H". iApply (wp_lift_pure_step_no_fork s E E'); try done.
   { naive_solver. }
   iApply (step_fupd_wand with "H"); iIntros "H".
-  iIntros (e' efs' σ (?&->&?)%Hpuredet); auto.
+  iIntros (α e' efs' σ (?&->&?)%Hpuredet); auto.
 Qed.
 
 Lemma wp_pure_step_fupd
